<?xml version="1.0"?>
<rdf:RDF xmlns="http://www.w3.org/2006/time#"
     xml:base="http://www.w3.org/2006/time"
     xmlns:dct="http://purl.org/dc/terms/"
     xmlns:owl="http://www.w3.org/2002/07/owl#"
     xmlns:rdf="http://www.w3.org/1999/02/22-rdf-syntax-ns#"
     xmlns:xml="http://www.w3.org/XML/1998/namespace"
     xmlns:xsd="http://www.w3.org/2001/XMLSchema#"
     xmlns:rdfs="http://www.w3.org/2000/01/rdf-schema#"
     xmlns:skos="http://www.w3.org/2004/02/skos/core#">
    <owl:Ontology rdf:about="http://www.w3.org/2006/time">
        <owl:versionIRI rdf:resource="http://www.w3.org/2006/time#2016"/>
        <dct:contributor rdf:resource="https://orcid.org/0000-0001-8269-8171"/>
        <dct:contributor rdf:resource="mailto:chris.little@metoffice.gov.uk"/>
        <dct:created rdf:datatype="http://www.w3.org/2001/XMLSchema#date">2006-09-27</dct:created>
        <dct:creator rdf:resource="http://orcid.org/0000-0002-3884-3420"/>
        <dct:creator rdf:resource="https://en.wikipedia.org/wiki/Jerry_Hobbs"/>
        <dct:creator rdf:resource="mailto:panfeng66@gmail.com"/>
        <dct:isVersionOf rdf:resource="http://www.w3.org/TR/owl-time"/>
        <dct:license rdf:resource="https://creativecommons.org/licenses/by/4.0/"/>
        <dct:modified rdf:datatype="http://www.w3.org/2001/XMLSchema#date">2017-04-06</dct:modified>
        <dct:rights xml:lang="en">Copyright � 2006-2017 W3C, OGC. W3C and OGC liability, trademark and document use rules apply.</dct:rights>
        <rdfs:label xml:lang="en">OWL-Time</rdfs:label>
        <rdfs:label xml:lang="es">Tiempo en OWL</rdfs:label>
        <rdfs:seeAlso rdf:resource="http://dx.doi.org/10.3233/SW-150187"/>
        <rdfs:seeAlso rdf:resource="http://www.semantic-web-journal.net/content/time-ontology-extended-non-gregorian-calendar-applications"/>
        <rdfs:seeAlso rdf:resource="http://www.w3.org/TR/owl-time"/>
        <owl:priorVersion rdf:resource="http://www.w3.org/2006/time#2006"/>
        <skos:changeNote>2016-06-15 - initial update of OWL-Time - modified to support arbitrary temporal reference systems. </skos:changeNote>
        <skos:changeNote>2016-12-20 - adjust range of time:timeZone to time:TimeZone, moved up from the tzont ontology.  </skos:changeNote>
        <skos:changeNote>2016-12-20 - restore time:Year and time:January which were present in the 2006 version of the ontology, but now marked &quot;deprecated&quot;. </skos:changeNote>
        <skos:changeNote>2017-02 - intervalIn, intervalDisjoint, monthOfYear added; TemporalUnit subclass of TemporalDuration</skos:changeNote>
        <skos:changeNote>2017-04-06 - hasTime, hasXSDDuration added; Number removed; all duration elements changed to xsd:decimal</skos:changeNote>
        <skos:historyNote xml:lang="en">Update of OWL-Time ontology, extended to support general temporal reference systems. 

Ontology engineering by Simon J D Cox</skos:historyNote>
    </owl:Ontology>
    


    <!-- 
    ///////////////////////////////////////////////////////////////////////////////////////
    //
    // Annotation properties
    //
    ///////////////////////////////////////////////////////////////////////////////////////
     -->

    


    <!-- http://purl.org/dc/terms/contributor -->

    <owl:AnnotationProperty rdf:about="http://purl.org/dc/terms/contributor"/>
    


    <!-- http://purl.org/dc/terms/created -->

    <owl:AnnotationProperty rdf:about="http://purl.org/dc/terms/created"/>
    


    <!-- http://purl.org/dc/terms/creator -->

    <owl:AnnotationProperty rdf:about="http://purl.org/dc/terms/creator"/>
    


    <!-- http://purl.org/dc/terms/isVersionOf -->

    <owl:AnnotationProperty rdf:about="http://purl.org/dc/terms/isVersionOf"/>
    


    <!-- http://purl.org/dc/terms/license -->

    <owl:AnnotationProperty rdf:about="http://purl.org/dc/terms/license"/>
    


    <!-- http://purl.org/dc/terms/modified -->

    <owl:AnnotationProperty rdf:about="http://purl.org/dc/terms/modified"/>
    


    <!-- http://purl.org/dc/terms/rights -->

    <owl:AnnotationProperty rdf:about="http://purl.org/dc/terms/rights"/>
    


    <!-- http://www.w3.org/2001/XMLSchema#pattern -->

    <owl:AnnotationProperty rdf:about="http://www.w3.org/2001/XMLSchema#pattern"/>
    


    <!-- http://www.w3.org/2004/02/skos/core#changeNote -->

    <owl:AnnotationProperty rdf:about="http://www.w3.org/2004/02/skos/core#changeNote"/>
    


    <!-- http://www.w3.org/2004/02/skos/core#definition -->

    <owl:AnnotationProperty rdf:about="http://www.w3.org/2004/02/skos/core#definition"/>
    


    <!-- http://www.w3.org/2004/02/skos/core#editorialNote -->

    <owl:AnnotationProperty rdf:about="http://www.w3.org/2004/02/skos/core#editorialNote"/>
    


    <!-- http://www.w3.org/2004/02/skos/core#historyNote -->

    <owl:AnnotationProperty rdf:about="http://www.w3.org/2004/02/skos/core#historyNote"/>
    


    <!-- http://www.w3.org/2004/02/skos/core#note -->

    <owl:AnnotationProperty rdf:about="http://www.w3.org/2004/02/skos/core#note"/>
    


    <!-- http://www.w3.org/2004/02/skos/core#prefLabel -->

    <owl:AnnotationProperty rdf:about="http://www.w3.org/2004/02/skos/core#prefLabel"/>
    


    <!-- http://www.w3.org/2004/02/skos/core#scopeNote -->

    <owl:AnnotationProperty rdf:about="http://www.w3.org/2004/02/skos/core#scopeNote"/>
    


    <!-- 
    ///////////////////////////////////////////////////////////////////////////////////////
    //
    // Datatypes
    //
    ///////////////////////////////////////////////////////////////////////////////////////
     -->

    


    <!-- http://www.w3.org/2001/XMLSchema#date -->

    <rdfs:Datatype rdf:about="http://www.w3.org/2001/XMLSchema#date"/>
    


    <!-- http://www.w3.org/2001/XMLSchema#dateTimeStamp -->

    <rdf:Description rdf:about="http://www.w3.org/2001/XMLSchema#dateTimeStamp">
        <rdfs:label xml:lang="es">sello de tiempo</rdfs:label>
    </rdf:Description>
    


    <!-- http://www.w3.org/2001/XMLSchema#duration -->

    <rdfs:Datatype rdf:about="http://www.w3.org/2001/XMLSchema#duration"/>
    


    <!-- http://www.w3.org/2001/XMLSchema#gDay -->

    <rdfs:Datatype rdf:about="http://www.w3.org/2001/XMLSchema#gDay"/>
    


    <!-- http://www.w3.org/2001/XMLSchema#gMonth -->

    <rdfs:Datatype rdf:about="http://www.w3.org/2001/XMLSchema#gMonth"/>
    


    <!-- http://www.w3.org/2001/XMLSchema#gYear -->

    <rdfs:Datatype rdf:about="http://www.w3.org/2001/XMLSchema#gYear"/>
    


    <!-- http://www.w3.org/2001/XMLSchema#gYearMonth -->

    <rdfs:Datatype rdf:about="http://www.w3.org/2001/XMLSchema#gYearMonth"/>
    


    <!-- http://www.w3.org/2006/time#generalDay -->

    <rdfs:Datatype rdf:about="http://www.w3.org/2006/time#generalDay">
        <rdfs:comment xml:lang="en">Day of month - formulated as a text string with a pattern constraint to reproduce the same lexical form as gDay, except that values up to 99 are permitted, in order to support calendars with more than 31 days in a month. 
Note that the value-space is not defined, so a generic OWL2 processor cannot compute ordering relationships of values of this type.</rdfs:comment>
        <rdfs:comment xml:lang="es">D�a del mes - formulado como una cadena de texto con una restricci�n patr�n para reproducir la misma forma l�xica que gDay, excepto que se permiten valores hasta el 99, con el prop�sito de proporcionar soporte a calendarios con meses con m�s de 31 d�as.
            N�tese que el espacio de valores no est� definido, por tanto, un procesador gen�rico de OWL2 no puede computar relaciones de orden de valores de este tipo.</rdfs:comment>
        <rdfs:label xml:lang="es">D�a generalizado</rdfs:label>
        <rdfs:label xml:lang="en">Generalized day</rdfs:label>
        <skos:definition xml:lang="en">Day of month - formulated as a text string with a pattern constraint to reproduce the same lexical form as gDay, except that values up to 99 are permitted, in order to support calendars with more than 31 days in a month. 
Note that the value-space is not defined, so a generic OWL2 processor cannot compute ordering relationships of values of this type.</skos:definition>
        <skos:definition xml:lang="es">D�a del mes - formulado como una cadena de texto con una restricci�n patr�n para reproducir la misma forma l�xica que gDay, excepto que se permiten valores hasta el 99, con el prop�sito de proporcionar soporte a calendarios con meses con m�s de 31 d�as.
            N�tese que el espacio de valores no est� definido, por tanto, un procesador gen�rico de OWL2 no puede computar relaciones de orden de valores de este tipo.</skos:definition>
    </rdfs:Datatype>
    


    <!-- http://www.w3.org/2006/time#generalMonth -->

    <rdfs:Datatype rdf:about="http://www.w3.org/2006/time#generalMonth">
        <rdfs:comment xml:lang="es">Mes del a�o - formulado como una cadena de texto con una restricci�n patr�n para reproducir la misma forma l�xica que gMonth, excepto que se permiten valores hasta el 20, con el prop�sito de proporcionar soporte a calendarios con a�os con m�s de 12 meses.
            N�tese que el espacio de valores no est� definido, por tanto, un procesador gen�rico de OWL2 no puede computar relaciones de orden de valores de este tipo.</rdfs:comment>
        <rdfs:comment xml:lang="en">Month of year - formulated as a text string with a pattern constraint to reproduce the same lexical form as gMonth, except that values up to 20 are permitted, in order to support calendars with more than 12 months in the year. 
Note that the value-space is not defined, so a generic OWL2 processor cannot compute ordering relationships of values of this type.</rdfs:comment>
        <rdfs:label xml:lang="en">Generalized month</rdfs:label>
        <rdfs:label xml:lang="es">Mes generalizado</rdfs:label>
        <skos:definition xml:lang="es">Mes del a�o - formulado como una cadena de texto con una restricci�n patr�n para reproducir la misma forma l�xica que gMonth, excepto que se permiten valores hasta el 20, con el prop�sito de proporcionar soporte a calendarios con a�os con m�s de 12 meses.
            N�tese que el espacio de valores no est� definido, por tanto, un procesador gen�rico de OWL2 no puede computar relaciones de orden de valores de este tipo.</skos:definition>
        <skos:definition xml:lang="en">Month of year - formulated as a text string with a pattern constraint to reproduce the same lexical form as gMonth, except that values up to 20 are permitted, in order to support calendars with more than 12 months in the year. 
Note that the value-space is not defined, so a generic OWL2 processor cannot compute ordering relationships of values of this type.</skos:definition>
    </rdfs:Datatype>
    


    <!-- http://www.w3.org/2006/time#generalYear -->

    <rdfs:Datatype rdf:about="http://www.w3.org/2006/time#generalYear">
        <rdfs:comment xml:lang="es">N�mero de a�o - formulado como una cadena de texto con una restricci�n patr�n para reproducir la misma forma l�xica que gYear, aunque no est� restringido a valores del calendario gregoriano.
            N�tese que el espacio de valores no est� definido, por tanto, un procesador gen�rico de OWL2 no puede computar relaciones de orden de valores de este tipo.</rdfs:comment>
        <rdfs:comment xml:lang="en">Year number - formulated as a text string with a pattern constraint to reproduce the same lexical form as gYear, but not restricted to values from the Gregorian calendar. 
Note that the value-space is not defined, so a generic OWL2 processor cannot compute ordering relationships of values of this type.</rdfs:comment>
        <rdfs:label xml:lang="es">A�o generalizado</rdfs:label>
        <rdfs:label xml:lang="en">Generalized year</rdfs:label>
        <skos:definition xml:lang="es">N�mero de a�o - formulado como una cadena de texto con una restricci�n patr�n para reproducir la misma forma l�xica que gYear, aunque no est� restringido a valores del calendario gregoriano.
            N�tese que el espacio de valores no est� definido, por tanto, un procesador gen�rico de OWL2 no puede computar relaciones de orden de valores de este tipo.</skos:definition>
        <skos:definition xml:lang="en">Year number - formulated as a text string with a pattern constraint to reproduce the same lexical form as gYear, but not restricted to values from the Gregorian calendar. 
Note that the value-space is not defined, so a generic OWL2 processor cannot compute ordering relationships of values of this type.</skos:definition>
    </rdfs:Datatype>
    


    <!-- 
    ///////////////////////////////////////////////////////////////////////////////////////
    //
    // Object Properties
    //
    ///////////////////////////////////////////////////////////////////////////////////////
     -->

    


    <!-- http://www.w3.org/2006/time#after -->

    <owl:ObjectProperty rdf:about="http://www.w3.org/2006/time#after">
        <owl:inverseOf rdf:resource="http://www.w3.org/2006/time#before"/>
        <rdfs:domain rdf:resource="http://www.w3.org/2006/time#TemporalEntity"/>
        <rdfs:range rdf:resource="http://www.w3.org/2006/time#TemporalEntity"/>
        <rdfs:comment xml:lang="es">Asume una direcci�n en el tiempo. Si una entidad temporal T1 est� despu�s de otra entidad temporal T2, entonces el principio de T1 est� despu�s del final de T2.</rdfs:comment>
        <rdfs:comment xml:lang="en">Gives directionality to time. If a temporal entity T1 is after another temporal entity T2, then the beginning of T1 is after the end of T2.</rdfs:comment>
        <rdfs:label xml:lang="en">after</rdfs:label>
        <rdfs:label xml:lang="es">despu�s</rdfs:label>
        <skos:definition xml:lang="es">Asume una direcci�n en el tiempo. Si una entidad temporal T1 est� despu�s de otra entidad temporal T2, entonces el principio de T1 est� despu�s del final de T2.</skos:definition>
        <skos:definition xml:lang="en">Gives directionality to time. If a temporal entity T1 is after another temporal entity T2, then the beginning of T1 is after the end of T2.</skos:definition>
    </owl:ObjectProperty>
    


    <!-- http://www.w3.org/2006/time#before -->

    <owl:ObjectProperty rdf:about="http://www.w3.org/2006/time#before">
        <rdf:type rdf:resource="http://www.w3.org/2002/07/owl#TransitiveProperty"/>
        <rdfs:domain rdf:resource="http://www.w3.org/2006/time#TemporalEntity"/>
        <rdfs:range rdf:resource="http://www.w3.org/2006/time#TemporalEntity"/>
        <rdfs:comment xml:lang="es">Asume una direcci�n en el tiempo. Si una entidad temporal T1 est� antes que otra entidad temporal T2, entonces el final de T1 est� antes que el principio de T2. As�, &quot;antes&quot; se puede considerar b�sica para instantes y derivada para intervalos.</rdfs:comment>
        <rdfs:comment xml:lang="en">Gives directionality to time. If a temporal entity T1 is before another temporal entity T2, then the end of T1 is before the beginning of T2. Thus, &quot;before&quot; can be considered to be basic to instants and derived for intervals.</rdfs:comment>
        <rdfs:label xml:lang="es">antes</rdfs:label>
        <rdfs:label xml:lang="en">before</rdfs:label>
        <skos:definition xml:lang="es">Asume una direcci�n en el tiempo. Si una entidad temporal T1 est� antes que otra entidad temporal T2, entonces el final de T1 est� antes que el principio de T2. As�, &quot;antes&quot; se puede considerar b�sica para instantes y derivada para intervalos.</skos:definition>
        <skos:definition xml:lang="en">Gives directionality to time. If a temporal entity T1 is before another temporal entity T2, then the end of T1 is before the beginning of T2. Thus, &quot;before&quot; can be considered to be basic to instants and derived for intervals.</skos:definition>
    </owl:ObjectProperty>
    


    <!-- http://www.w3.org/2006/time#dayOfWeek -->

    <owl:ObjectProperty rdf:about="http://www.w3.org/2006/time#dayOfWeek">
        <rdfs:domain rdf:resource="http://www.w3.org/2006/time#GeneralDateTimeDescription"/>
        <rdfs:range rdf:resource="http://www.w3.org/2006/time#DayOfWeek"/>
        <rdfs:comment>El d�a de la semana, cuyo valor es un miembro de la clase &apos;d�a de la semana&apos;.</rdfs:comment>
        <rdfs:comment xml:lang="en">The day of week, whose value is a member of the class time:DayOfWeek</rdfs:comment>
        <rdfs:label xml:lang="en">day of week</rdfs:label>
        <rdfs:label xml:lang="es">d�a de la semana</rdfs:label>
        <skos:definition xml:lang="es">El d�a de la semana, cuyo valor es un miembro de la clase &apos;d�a de la semana&apos;.</skos:definition>
        <skos:definition xml:lang="en">The day of week, whose value is a member of the class time:DayOfWeek</skos:definition>
    </owl:ObjectProperty>
    


    <!-- http://www.w3.org/2006/time#hasBeginning -->

    <owl:ObjectProperty rdf:about="http://www.w3.org/2006/time#hasBeginning">
        <rdfs:subPropertyOf rdf:resource="http://www.w3.org/2006/time#hasTime"/>
        <rdfs:domain rdf:resource="http://www.w3.org/2006/time#TemporalEntity"/>
        <rdfs:range rdf:resource="http://www.w3.org/2006/time#Instant"/>
        <rdfs:comment xml:lang="en">Beginning of a temporal entity</rdfs:comment>
        <rdfs:comment xml:lang="es">Comienzo de una entidad temporal.</rdfs:comment>
        <rdfs:label xml:lang="en">has beginning</rdfs:label>
        <rdfs:label xml:lang="es">tiene principio</rdfs:label>
        <skos:definition xml:lang="en">Beginning of a temporal entity.</skos:definition>
        <skos:definition xml:lang="es">Comienzo de una entidad temporal.</skos:definition>
    </owl:ObjectProperty>
    


    <!-- http://www.w3.org/2006/time#hasDateTimeDescription -->

    <owl:ObjectProperty rdf:about="http://www.w3.org/2006/time#hasDateTimeDescription">
        <rdfs:domain rdf:resource="http://www.w3.org/2006/time#DateTimeInterval"/>
        <rdfs:range rdf:resource="http://www.w3.org/2006/time#GeneralDateTimeDescription"/>
        <rdfs:comment xml:lang="es">Valor de intervalo de fecha-hora expresado como un valor estructurado. El principio y el final del intervalo coincide con los l�mites del elemento m�s corto en la descripci�n.</rdfs:comment>
        <rdfs:comment xml:lang="en">Value of DateTimeInterval expressed as a structured value. The beginning and end of the interval coincide with the limits of the shortest element in the description.</rdfs:comment>
        <rdfs:label xml:lang="en">has Date-Time description</rdfs:label>
        <rdfs:label xml:lang="es">tiene descripci�n fecha-hora</rdfs:label>
        <skos:definition xml:lang="es">Valor de intervalo de fecha-hora expresado como un valor estructurado. El principio y el final del intervalo coincide con los l�mites del elemento m�s corto en la descripci�n.</skos:definition>
        <skos:definition xml:lang="en">Value of DateTimeInterval expressed as a structured value. The beginning and end of the interval coincide with the limits of the shortest element in the description.</skos:definition>
    </owl:ObjectProperty>
    


    <!-- http://www.w3.org/2006/time#hasDuration -->

    <owl:ObjectProperty rdf:about="http://www.w3.org/2006/time#hasDuration">
        <rdfs:subPropertyOf rdf:resource="http://www.w3.org/2006/time#hasTemporalDuration"/>
        <rdfs:range rdf:resource="http://www.w3.org/2006/time#Duration"/>
        <rdfs:comment xml:lang="es">Duraci�n de una entidad temporal, expresada como un valor escalado o un valor nominal.</rdfs:comment>
        <rdfs:comment xml:lang="en">Duration of a temporal entity, expressed as a scaled value or nominal value</rdfs:comment>
        <rdfs:label xml:lang="en">has duration</rdfs:label>
        <rdfs:label xml:lang="es">tiene duraci�n</rdfs:label>
        <skos:definition xml:lang="es">Duraci�n de una entidad temporal, evento o actividad, o cosa, expresada como un valor escalado.</skos:definition>
        <skos:definition xml:lang="en">Duration of a temporal entity, event or activity, or thing, expressed as a scaled value</skos:definition>
    </owl:ObjectProperty>
    


    <!-- http://www.w3.org/2006/time#hasDurationDescription -->

    <owl:ObjectProperty rdf:about="http://www.w3.org/2006/time#hasDurationDescription">
        <rdfs:subPropertyOf rdf:resource="http://www.w3.org/2006/time#hasTemporalDuration"/>
        <rdfs:range rdf:resource="http://www.w3.org/2006/time#GeneralDurationDescription"/>
        <rdfs:comment xml:lang="es">Duraci�n de una entidad temporal, expresada utilizando una descripci�n estructurada.</rdfs:comment>
        <rdfs:comment xml:lang="en">Duration of a temporal entity, expressed using a structured description</rdfs:comment>
        <rdfs:label xml:lang="en">has duration description</rdfs:label>
        <rdfs:label xml:lang="es">tiene descripci�n de duraci�n</rdfs:label>
        <skos:definition xml:lang="es">Duraci�n de una entidad temporal, expresada utilizando una descripci�n estructurada.</skos:definition>
        <skos:definition xml:lang="en">Duration of a temporal entity, expressed using a structured description</skos:definition>
    </owl:ObjectProperty>
    


    <!-- http://www.w3.org/2006/time#hasEnd -->

    <owl:ObjectProperty rdf:about="http://www.w3.org/2006/time#hasEnd">
        <rdfs:subPropertyOf rdf:resource="http://www.w3.org/2006/time#hasTime"/>
        <rdfs:domain rdf:resource="http://www.w3.org/2006/time#TemporalEntity"/>
        <rdfs:range rdf:resource="http://www.w3.org/2006/time#Instant"/>
        <rdfs:comment xml:lang="en">End of a temporal entity.</rdfs:comment>
        <rdfs:comment xml:lang="es">Final de una entidad temporal.</rdfs:comment>
        <rdfs:label xml:lang="en">has end</rdfs:label>
        <rdfs:label xml:lang="es">tiene fin</rdfs:label>
        <skos:definition xml:lang="en">End of a temporal entity.</skos:definition>
        <skos:definition xml:lang="es">Final de una entidad temporal.</skos:definition>
    </owl:ObjectProperty>
    


    <!-- http://www.w3.org/2006/time#hasTRS -->

    <owl:ObjectProperty rdf:about="http://www.w3.org/2006/time#hasTRS">
        <rdf:type rdf:resource="http://www.w3.org/2002/07/owl#FunctionalProperty"/>
        <rdfs:domain>
            <owl:Class>
                <owl:unionOf rdf:parseType="Collection">
                    <rdf:Description rdf:about="http://www.w3.org/2006/time#GeneralDurationDescription"/>
                    <rdf:Description rdf:about="http://www.w3.org/2006/time#TemporalPosition"/>
                </owl:unionOf>
            </owl:Class>
        </rdfs:domain>
        <rdfs:range rdf:resource="http://www.w3.org/2006/time#TRS"/>
        <rdfs:comment xml:lang="es">El sistema de referencia temporal utilizado por una posici�n temporal o descripci�n de extensi�n.</rdfs:comment>
        <rdfs:comment xml:lang="en">The temporal reference system used by a temporal position or extent description. </rdfs:comment>
        <rdfs:label xml:lang="en">Temporal reference system used</rdfs:label>
        <rdfs:label xml:lang="es">sistema de referencia temporal utilizado</rdfs:label>
        <skos:definition xml:lang="es">El sistema de referencia temporal utilizado por una posici�n temporal o descripci�n de extensi�n.</skos:definition>
        <skos:definition xml:lang="en">The temporal reference system used by a temporal position or extent description. </skos:definition>
    </owl:ObjectProperty>
    


    <!-- http://www.w3.org/2006/time#hasTemporalDuration -->

    <owl:ObjectProperty rdf:about="http://www.w3.org/2006/time#hasTemporalDuration">
        <rdfs:domain rdf:resource="http://www.w3.org/2006/time#TemporalEntity"/>
        <rdfs:range rdf:resource="http://www.w3.org/2006/time#TemporalDuration"/>
        <rdfs:comment xml:lang="es">Duraci�n de una entidad temporal.</rdfs:comment>
        <rdfs:comment xml:lang="en">Duration of a temporal entity.</rdfs:comment>
        <rdfs:label xml:lang="en">has temporal duration</rdfs:label>
        <rdfs:label xml:lang="es">tiene duraci�n temporal</rdfs:label>
        <skos:definition xml:lang="es">Duraci�n de una entidad temporal.</skos:definition>
        <skos:definition xml:lang="en">Duration of a temporal entity.</skos:definition>
    </owl:ObjectProperty>
    


    <!-- http://www.w3.org/2006/time#hasTime -->

    <owl:ObjectProperty rdf:about="http://www.w3.org/2006/time#hasTime">
        <rdfs:range rdf:resource="http://www.w3.org/2006/time#TemporalEntity"/>
        <rdfs:comment xml:lang="es">Proporciona soporte a la asociaci�n de una entidad temporal (instante o intervalo) a cualquier cosa.</rdfs:comment>
        <rdfs:comment xml:lang="en">Supports the association of a temporal entity (instant or interval) to any thing</rdfs:comment>
        <rdfs:label xml:lang="en">has time</rdfs:label>
        <rdfs:label xml:lang="es">tiene tiempo</rdfs:label>
        <skos:definition xml:lang="es">Proporciona soporte a la asociaci�n de una entidad temporal (instante o intervalo) a cualquier cosa.</skos:definition>
        <skos:definition xml:lang="en">Supports the association of a temporal entity (instant or interval) to any thing</skos:definition>
        <skos:editorialNote xml:lang="es">Caracter�stica arriesgada -a�adida en la revisi�n del 2017 que no ha sido todav�a utilizada de forma amplia.</skos:editorialNote>
        <skos:editorialNote xml:lang="en">Feature at risk - added in 2017 revision, and not yet widely used. </skos:editorialNote>
    </owl:ObjectProperty>
    


    <!-- http://www.w3.org/2006/time#inDateTime -->

    <owl:ObjectProperty rdf:about="http://www.w3.org/2006/time#inDateTime">
        <rdfs:subPropertyOf rdf:resource="http://www.w3.org/2006/time#inTemporalPosition"/>
        <rdfs:domain rdf:resource="http://www.w3.org/2006/time#Instant"/>
        <rdfs:range rdf:resource="http://www.w3.org/2006/time#GeneralDateTimeDescription"/>
        <rdfs:comment xml:lang="es">Posici�n de un instante, expresada utilizando una descripci�n estructurada.</rdfs:comment>
        <rdfs:comment xml:lang="en">Position of an instant, expressed using a structured description</rdfs:comment>
        <rdfs:label xml:lang="es">en descripci�n de fecha-hora</rdfs:label>
        <rdfs:label xml:lang="en">in date-time description</rdfs:label>
        <skos:definition xml:lang="es">Posici�n de un instante, expresada utilizando una descripci�n estructurada.</skos:definition>
        <skos:definition xml:lang="en">Position of an instant, expressed using a structured description</skos:definition>
    </owl:ObjectProperty>
    


    <!-- http://www.w3.org/2006/time#inTemporalPosition -->

    <owl:ObjectProperty rdf:about="http://www.w3.org/2006/time#inTemporalPosition">
        <rdfs:domain rdf:resource="http://www.w3.org/2006/time#Instant"/>
        <rdfs:range rdf:resource="http://www.w3.org/2006/time#TemporalPosition"/>
        <rdfs:comment xml:lang="es">Posici�n de un instante de tiempo.</rdfs:comment>
        <rdfs:comment xml:lang="en">Position of a time instant</rdfs:comment>
        <rdfs:label xml:lang="en">Temporal position</rdfs:label>
        <rdfs:label xml:lang="es">posici�n temporal</rdfs:label>
        <skos:definition xml:lang="es">Posici�n de un instante de tiempo.</skos:definition>
        <skos:definition xml:lang="en">Position of a time instant</skos:definition>
    </owl:ObjectProperty>
    


    <!-- http://www.w3.org/2006/time#inTimePosition -->

    <owl:ObjectProperty rdf:about="http://www.w3.org/2006/time#inTimePosition">
        <rdfs:subPropertyOf rdf:resource="http://www.w3.org/2006/time#inTemporalPosition"/>
        <rdfs:domain rdf:resource="http://www.w3.org/2006/time#Instant"/>
        <rdfs:range rdf:resource="http://www.w3.org/2006/time#TimePosition"/>
        <rdfs:comment xml:lang="es">Posici�n de un instante, expresada como una coordenada temporal o un valor nominal.</rdfs:comment>
        <rdfs:comment xml:lang="en">Position of an instant, expressed as a temporal coordinate or nominal value</rdfs:comment>
        <rdfs:label xml:lang="en">Time position</rdfs:label>
        <rdfs:label xml:lang="es">posici�n de tiempo</rdfs:label>
        <skos:definition xml:lang="es">Posici�n de un instante, expresada como una coordenada temporal o un valor nominal.</skos:definition>
        <skos:definition xml:lang="en">Position of a time instant expressed as a TimePosition</skos:definition>
    </owl:ObjectProperty>
    


    <!-- http://www.w3.org/2006/time#inside -->

    <owl:ObjectProperty rdf:about="http://www.w3.org/2006/time#inside">
        <rdfs:domain rdf:resource="http://www.w3.org/2006/time#Interval"/>
        <rdfs:range rdf:resource="http://www.w3.org/2006/time#Instant"/>
        <rdfs:comment xml:lang="en">An instant that falls inside the interval. It is not intended to include beginnings and ends of intervals.</rdfs:comment>
        <rdfs:comment xml:lang="es">Un instante que cae dentro del intervalo. Se asume que no es ni el principio ni el final de ning�n intervalo.</rdfs:comment>
        <rdfs:label xml:lang="en">has time instant inside</rdfs:label>
        <rdfs:label xml:lang="es">tiene instante de tiempo dentro</rdfs:label>
        <skos:definition xml:lang="en">An instant that falls inside the interval. It is not intended to include beginnings and ends of intervals.</skos:definition>
        <skos:definition xml:lang="es">Un instante que cae dentro del intervalo. Se asume que no es ni el principio ni el final de ning�n intervalo.</skos:definition>
    </owl:ObjectProperty>
    


    <!-- http://www.w3.org/2006/time#intervalAfter -->

    <owl:ObjectProperty rdf:about="http://www.w3.org/2006/time#intervalAfter">
        <rdfs:subPropertyOf rdf:resource="http://www.w3.org/2006/time#after"/>
        <rdfs:subPropertyOf rdf:resource="http://www.w3.org/2006/time#intervalDisjoint"/>
        <owl:inverseOf rdf:resource="http://www.w3.org/2006/time#intervalBefore"/>
        <rdfs:domain rdf:resource="http://www.w3.org/2006/time#ProperInterval"/>
        <rdfs:range rdf:resource="http://www.w3.org/2006/time#ProperInterval"/>
        <rdfs:comment xml:lang="en">If a proper interval T1 is intervalAfter another proper interval T2, then the beginning of T1 is after the end of T2.</rdfs:comment>
        <rdfs:comment>Si un intervalo propio T1 es posterior a otro intervalo propio T2, entonces el principio de T1 est� despu�s que el final de T2.</rdfs:comment>
        <rdfs:label xml:lang="en">interval after</rdfs:label>
        <rdfs:label xml:lang="es">intervalo posterior</rdfs:label>
        <skos:definition xml:lang="en">If a proper interval T1 is intervalAfter another proper interval T2, then the beginning of T1 is after the end of T2.</skos:definition>
        <skos:definition xml:lang="es">Si un intervalo propio T1 es posterior a otro intervalo propio T2, entonces el principio de T1 est� despu�s que el final de T2.</skos:definition>
    </owl:ObjectProperty>
    


    <!-- http://www.w3.org/2006/time#intervalBefore -->

    <owl:ObjectProperty rdf:about="http://www.w3.org/2006/time#intervalBefore">
        <rdfs:subPropertyOf rdf:resource="http://www.w3.org/2006/time#before"/>
        <rdfs:subPropertyOf rdf:resource="http://www.w3.org/2006/time#intervalDisjoint"/>
        <rdfs:domain rdf:resource="http://www.w3.org/2006/time#ProperInterval"/>
        <rdfs:range rdf:resource="http://www.w3.org/2006/time#ProperInterval"/>
        <rdfs:comment xml:lang="en">If a proper interval T1 is intervalBefore another proper interval T2, then the end of T1 is before the beginning of T2.</rdfs:comment>
        <rdfs:comment xml:lang="es">Si un intervalo propio T1 est� antes que otro intervalo propio T2, entonces el final de T1 est� antes que el principio de T2.</rdfs:comment>
        <rdfs:label xml:lang="en">interval before</rdfs:label>
        <rdfs:label xml:lang="es">intervalo anterior</rdfs:label>
        <skos:definition xml:lang="en">If a proper interval T1 is intervalBefore another proper interval T2, then the end of T1 is before the beginning of T2.</skos:definition>
        <skos:definition xml:lang="es">Si un intervalo propio T1 est� antes que otro intervalo propio T2, entonces el final de T1 est� antes que el principio de T2.</skos:definition>
    </owl:ObjectProperty>
    


    <!-- http://www.w3.org/2006/time#intervalContains -->

    <owl:ObjectProperty rdf:about="http://www.w3.org/2006/time#intervalContains">
        <owl:inverseOf rdf:resource="http://www.w3.org/2006/time#intervalDuring"/>
        <rdfs:domain rdf:resource="http://www.w3.org/2006/time#ProperInterval"/>
        <rdfs:range rdf:resource="http://www.w3.org/2006/time#ProperInterval"/>
        <rdfs:comment xml:lang="en">If a proper interval T1 is intervalContains another proper interval T2, then the beginning of T1 is before the beginning of T2, and the end of T1 is after the end of T2.</rdfs:comment>
        <rdfs:comment xml:lang="es">Si un intervalo propio T1 contiene otro intervalo propio T2, entonces el principio de T1 est� antes que el principio de T2, y el final de T1 est� despu�s del final de T2.</rdfs:comment>
        <rdfs:label xml:lang="en">interval contains</rdfs:label>
        <rdfs:label xml:lang="es">intervalo contiene</rdfs:label>
        <skos:definition xml:lang="en">If a proper interval T1 is intervalContains another proper interval T2, then the beginning of T1 is before the beginning of T2, and the end of T1 is after the end of T2.</skos:definition>
        <skos:definition xml:lang="es">Si un intervalo propio T1 contiene otro intervalo propio T2, entonces el principio de T1 est� antes que el principio de T2, y el final de T1 est� despu�s del final de T2.</skos:definition>
    </owl:ObjectProperty>
    


    <!-- http://www.w3.org/2006/time#intervalDisjoint -->

    <owl:ObjectProperty rdf:about="http://www.w3.org/2006/time#intervalDisjoint">
        <rdfs:domain rdf:resource="http://www.w3.org/2006/time#ProperInterval"/>
        <rdfs:range rdf:resource="http://www.w3.org/2006/time#ProperInterval"/>
        <rdfs:comment xml:lang="en">If a proper interval T1 is intervalDisjoint another proper interval T2, then the beginning of T1 is after the end of T2, or the end of T1 is before the beginning of T2, i.e. the intervals do not overlap in any way, but their ordering relationship is not known.</rdfs:comment>
        <rdfs:comment xml:lang="es">Si un intervalo propio T1 es disjunto con otro intervalo propio T2, entonces el principio de T1 est� despu�s del final de T2, o el final de T1 est� antes que el principio de T2, es decir, los intervalos no se solapan de ninguna forma, aunque su relaci�n de orden no se conozca.</rdfs:comment>
        <rdfs:label xml:lang="en">interval disjoint</rdfs:label>
        <rdfs:label xml:lang="es">intervalo disjunto</rdfs:label>
        <skos:definition xml:lang="en">If a proper interval T1 is intervalDisjoint another proper interval T2, then the beginning of T1 is after the end of T2, or the end of T1 is before the beginning of T2, i.e. the intervals do not overlap in any way, but their ordering relationship is not known.</skos:definition>
        <skos:definition xml:lang="es">Si un intervalo propio T1 es disjunto con otro intervalo propio T2, entonces el principio de T1 est� despu�s del final de T2, o el final de T1 est� antes que el principio de T2, es decir, los intervalos no se solapan de ninguna forma, aunque su relaci�n de orden no se conozca.</skos:definition>
        <skos:note xml:lang="es">Esta relaci�n entre intervalos no estaba incluida en las 13 relaciones b�sicas definidas por Allen (1984), pero est� definida en T.3 como la uni�n de &apos;intervalo anterior&apos; con &apos;intervalo posterior&apos;. Sin embargo, esto est� fuera de la expresividad de OWL2, por tanto, est� implementado como una propiedad expl�cita, con &apos;intervalo anterior&apos; e &apos;intervalo posterior&apos; como sub-propiedades.</skos:note>
        <skos:note xml:lang="en">This interval relation is not included in the 13 basic relationships defined in Allen (1984), but is defined in (T.3) as the union of :intervalBefore v :intervalAfter . However, that is outside OWL2 expressivity, so is implemented as an explicit property, with :intervalBefore , :intervalAfter as sub-properties</skos:note>
    </owl:ObjectProperty>
    


    <!-- http://www.w3.org/2006/time#intervalDuring -->

    <owl:ObjectProperty rdf:about="http://www.w3.org/2006/time#intervalDuring">
        <rdfs:subPropertyOf rdf:resource="http://www.w3.org/2006/time#intervalIn"/>
        <rdfs:domain rdf:resource="http://www.w3.org/2006/time#ProperInterval"/>
        <rdfs:range rdf:resource="http://www.w3.org/2006/time#ProperInterval"/>
        <rdfs:comment xml:lang="en">If a proper interval T1 is intervalDuring another proper interval T2, then the beginning of T1 is after the beginning of T2, and the end of T1 is before the end of T2.</rdfs:comment>
        <rdfs:comment xml:lang="es">Si un intervalo propio T1 est� durante otro intervalo propio T2, entonces del principio de T1 est� despu�s del principio de T2, y el final de T1 est� antes que el final de T2.</rdfs:comment>
        <rdfs:label xml:lang="en">interval during</rdfs:label>
        <rdfs:label xml:lang="es">intervalo durante</rdfs:label>
        <skos:definition xml:lang="en">If a proper interval T1 is intervalDuring another proper interval T2, then the beginning of T1 is after the beginning of T2, and the end of T1 is before the end of T2.</skos:definition>
        <skos:definition xml:lang="es">Si un intervalo propio T1 est� durante otro intervalo propio T2, entonces del principio de T1 est� despu�s del principio de T2, y el final de T1 est� antes que el final de T2.</skos:definition>
    </owl:ObjectProperty>
    


    <!-- http://www.w3.org/2006/time#intervalEquals -->

    <owl:ObjectProperty rdf:about="http://www.w3.org/2006/time#intervalEquals">
        <rdfs:domain rdf:resource="http://www.w3.org/2006/time#ProperInterval"/>
        <rdfs:range rdf:resource="http://www.w3.org/2006/time#ProperInterval"/>
        <owl:propertyDisjointWith rdf:resource="http://www.w3.org/2006/time#intervalIn"/>
        <rdfs:comment xml:lang="en">If a proper interval T1 is intervalEquals another proper interval T2, then the beginning of T1 is coincident with the beginning of T2, and the end of T1 is coincident with the end of T2.</rdfs:comment>
        <rdfs:comment xml:lang="es">Si un intervalo propio T1 es igual a otro intervalo propio T2, entonces el principio de T1 coincide con el principio de T2, y el final de T1 coincide con el final de T2.</rdfs:comment>
        <rdfs:label xml:lang="en">interval equals</rdfs:label>
        <rdfs:label xml:lang="es">intervalo igual</rdfs:label>
        <skos:definition xml:lang="en">If a proper interval T1 is intervalEquals another proper interval T2, then the beginning of T1 is coincident with the beginning of T2, and the end of T1 is coincident with the end of T2.</skos:definition>
        <skos:definition xml:lang="es">Si un intervalo propio T1 es igual a otro intervalo propio T2, entonces el principio de T1 coincide con el principio de T2, y el final de T1 coincide con el final de T2.</skos:definition>
    </owl:ObjectProperty>
    


    <!-- http://www.w3.org/2006/time#intervalFinishedBy -->

    <owl:ObjectProperty rdf:about="http://www.w3.org/2006/time#intervalFinishedBy">
        <owl:inverseOf rdf:resource="http://www.w3.org/2006/time#intervalFinishes"/>
        <rdfs:domain rdf:resource="http://www.w3.org/2006/time#ProperInterval"/>
        <rdfs:range rdf:resource="http://www.w3.org/2006/time#ProperInterval"/>
        <rdfs:comment xml:lang="en">If a proper interval T1 is intervalFinishedBy another proper interval T2, then the beginning of T1 is before the beginning of T2, and the end of T1 is coincident with the end of T2.</rdfs:comment>
        <rdfs:comment xml:lang="es">Si un intervalo propio T1 est� terminado por otro intervalo propio T2, entonces el principio de T1 est� antes que el principio de T2, y el final de T1 coincide con el final de T2.</rdfs:comment>
        <rdfs:label xml:lang="en">interval finished by</rdfs:label>
        <rdfs:label xml:lang="es">intervalo terminado por</rdfs:label>
        <skos:definition xml:lang="en">If a proper interval T1 is intervalFinishedBy another proper interval T2, then the beginning of T1 is before the beginning of T2, and the end of T1 is coincident with the end of T2.</skos:definition>
        <skos:definition xml:lang="es">Si un intervalo propio T1 est� terminado por otro intervalo propio T2, entonces el principio de T1 est� antes que el principio de T2, y el final de T1 coincide con el final de T2.</skos:definition>
    </owl:ObjectProperty>
    


    <!-- http://www.w3.org/2006/time#intervalFinishes -->

    <owl:ObjectProperty rdf:about="http://www.w3.org/2006/time#intervalFinishes">
        <rdfs:subPropertyOf rdf:resource="http://www.w3.org/2006/time#intervalIn"/>
        <rdfs:domain rdf:resource="http://www.w3.org/2006/time#ProperInterval"/>
        <rdfs:range rdf:resource="http://www.w3.org/2006/time#ProperInterval"/>
        <rdfs:comment xml:lang="en">If a proper interval T1 is intervalFinishes another proper interval T2, then the beginning of T1 is after the beginning of T2, and the end of T1 is coincident with the end of T2.</rdfs:comment>
        <rdfs:comment xml:lang="es">Si un intervalo propio T1 termina otro intervalo propio T2, entonces del principio de T1 est� despu�s del principio de T2, y el final de T1 coincide con el final de T2.</rdfs:comment>
        <rdfs:label xml:lang="en">interval finishes</rdfs:label>
        <rdfs:label xml:lang="es">intervalo termina</rdfs:label>
        <skos:definition xml:lang="en">If a proper interval T1 is intervalFinishes another proper interval T2, then the beginning of T1 is after the beginning of T2, and the end of T1 is coincident with the end of T2.</skos:definition>
        <skos:definition xml:lang="es">Si un intervalo propio T1 termina otro intervalo propio T2, entonces del principio de T1 est� despu�s del principio de T2, y el final de T1 coincide con el final de T2.</skos:definition>
    </owl:ObjectProperty>
    


    <!-- http://www.w3.org/2006/time#intervalIn -->

    <owl:ObjectProperty rdf:about="http://www.w3.org/2006/time#intervalIn">
        <rdfs:domain rdf:resource="http://www.w3.org/2006/time#ProperInterval"/>
        <rdfs:range rdf:resource="http://www.w3.org/2006/time#ProperInterval"/>
        <rdfs:comment xml:lang="en">If a proper interval T1 is intervalIn another proper interval T2, then the beginning of T1 is after the beginning of T2 or is coincident with the beginning of T2, and the end of T1 is before the end of T2, or is coincident with the end of T2, except that end of T1 may not be coincident with the end of T2 if the beginning of T1 is coincident with the beginning of T2.</rdfs:comment>
        <rdfs:comment xml:lang="es">Si un intervalo propio T1 es un intervalo interior a otro intervalo propio T2, entonces el principio de T1 est� despu�s del principio de T2 o coincide con el principio de T2, y el final de T1 est� antes que el final de T2, o coincide con el final de T2, excepto que el final de T1 puede no coincidir con el final de T2 si el principio de T1 coincide con el principio de T2.</rdfs:comment>
        <rdfs:label xml:lang="en">interval in</rdfs:label>
        <rdfs:label xml:lang="es">intervalo interior</rdfs:label>
        <skos:definition xml:lang="en">If a proper interval T1 is intervalIn another proper interval T2, then the beginning of T1 is after the beginning of T2 or is coincident with the beginning of T2, and the end of T1 is before the end of T2, or is coincident with the end of T2, except that end of T1 may not be coincident with the end of T2 if the beginning of T1 is coincident with the beginning of T2.</skos:definition>
        <skos:definition xml:lang="es">Si un intervalo propio T1 es un intervalo interior a otro intervalo propio T2, entonces el principio de T1 est� despu�s del principio de T2 o coincide con el principio de T2, y el final de T1 est� antes que el final de T2, o coincide con el final de T2, excepto que el final de T1 puede no coincidir con el final de T2 si el principio de T1 coincide con el principio de T2.</skos:definition>
        <skos:note xml:lang="es">Esta relaci�n entre intervalos no estaba incluida en las 13 relaciones b�sicas definidas por Allen (1984), pero se hace referencia a ella como &quot;una relaci�n importante&quot; en Allen y Ferguson (1997). Es la uni�n disjunta de &apos;intervalo empieza&apos;, &apos;intervalo durante&apos; y con &apos;intervalo termina&apos;. Sin embargo, esto est� fuera de la expresividad de OWL2, por tanto, se implementa como una propiedad expl�cita, con &apos;intervalo empieza&apos;, &apos;intervalo durante&apos; e &apos;intervalo termina&apos; como sub-propiedades.</skos:note>
        <skos:note xml:lang="en">This interval relation is not included in the 13 basic relationships defined in Allen (1984), but is referred to as &apos;an important relationship&apos; in Allen and Ferguson (1997). It is the disjoint union of :intervalStarts v :intervalDuring v :intervalFinishes . However, that is outside OWL2 expressivity, so is implemented as an explicit property, with :intervalStarts , :intervalDuring , :intervalFinishes as sub-properties</skos:note>
    </owl:ObjectProperty>
    


    <!-- http://www.w3.org/2006/time#intervalMeets -->

    <owl:ObjectProperty rdf:about="http://www.w3.org/2006/time#intervalMeets">
        <owl:inverseOf rdf:resource="http://www.w3.org/2006/time#intervalMetBy"/>
        <rdfs:domain rdf:resource="http://www.w3.org/2006/time#ProperInterval"/>
        <rdfs:range rdf:resource="http://www.w3.org/2006/time#ProperInterval"/>
        <rdfs:comment xml:lang="en">If a proper interval T1 is intervalMeets another proper interval T2, then the end of T1 is coincident with the beginning of T2.</rdfs:comment>
        <rdfs:comment xml:lang="es">Si un intervalo propio T1 se encuentra con otro intervalo propio T2, entonces el final de T1 coincide con el principio de T2.</rdfs:comment>
        <rdfs:label xml:lang="en">interval meets</rdfs:label>
        <rdfs:label xml:lang="es">intervalo se encuentra</rdfs:label>
        <skos:definition xml:lang="en">If a proper interval T1 is intervalMeets another proper interval T2, then the end of T1 is coincident with the beginning of T2.</skos:definition>
        <skos:definition xml:lang="es">Si un intervalo propio T1 se encuentra con otro intervalo propio T2, entonces el final de T1 coincide con el principio de T2.</skos:definition>
    </owl:ObjectProperty>
    


    <!-- http://www.w3.org/2006/time#intervalMetBy -->

    <owl:ObjectProperty rdf:about="http://www.w3.org/2006/time#intervalMetBy">
        <rdfs:domain rdf:resource="http://www.w3.org/2006/time#ProperInterval"/>
        <rdfs:range rdf:resource="http://www.w3.org/2006/time#ProperInterval"/>
        <rdfs:comment xml:lang="en">If a proper interval T1 is intervalMetBy another proper interval T2, then the beginning of T1 is coincident with the end of T2.</rdfs:comment>
        <rdfs:comment xml:lang="es">Si un intervalo propio T1 es &apos;intervalo encontrado por&apos; otro intervalo propio T2, entonces el principio de T1 coincide con el final de T2.</rdfs:comment>
        <rdfs:label xml:lang="en">interval met by</rdfs:label>
        <rdfs:label xml:lang="es">intervalo encontrado por</rdfs:label>
        <skos:definition xml:lang="en">If a proper interval T1 is intervalMetBy another proper interval T2, then the beginning of T1 is coincident with the end of T2.</skos:definition>
        <skos:definition xml:lang="es">Si un intervalo propio T1 es &apos;intervalo encontrado por&apos; otro intervalo propio T2, entonces el principio de T1 coincide con el final de T2.</skos:definition>
    </owl:ObjectProperty>
    


    <!-- http://www.w3.org/2006/time#intervalOverlappedBy -->

    <owl:ObjectProperty rdf:about="http://www.w3.org/2006/time#intervalOverlappedBy">
        <owl:inverseOf rdf:resource="http://www.w3.org/2006/time#intervalOverlaps"/>
        <rdfs:domain rdf:resource="http://www.w3.org/2006/time#ProperInterval"/>
        <rdfs:range rdf:resource="http://www.w3.org/2006/time#ProperInterval"/>
        <rdfs:comment xml:lang="en">If a proper interval T1 is intervalOverlappedBy another proper interval T2, then the beginning of T1 is after the beginning of T2, the beginning of T1 is before the end of T2, and the end of T1 is after the end of T2.</rdfs:comment>
        <rdfs:comment xml:lang="es">Si un intervalo propio T1 es &apos;intervalo solapado por&apos; otro intervalo propio T2, entonces el principio de T1 es posterior al principio de T2, y el principio de T1 es anterior al final de T2, y el final de T1 es posterior al final de T2.</rdfs:comment>
        <rdfs:label xml:lang="en">interval overlapped by</rdfs:label>
        <rdfs:label xml:lang="es">intervalo solapado por</rdfs:label>
        <skos:definition xml:lang="en">If a proper interval T1 is intervalOverlappedBy another proper interval T2, then the beginning of T1 is after the beginning of T2, the beginning of T1 is before the end of T2, and the end of T1 is after the end of T2.</skos:definition>
        <skos:definition xml:lang="es">Si un intervalo propio T1 es &apos;intervalo solapado por&apos; otro intervalo propio T2, entonces el principio de T1 es posterior al principio de T2, y el principio de T1 es anterior al final de T2, y el final de T1 es posterior al final de T2.</skos:definition>
    </owl:ObjectProperty>
    


    <!-- http://www.w3.org/2006/time#intervalOverlaps -->

    <owl:ObjectProperty rdf:about="http://www.w3.org/2006/time#intervalOverlaps">
        <rdfs:domain rdf:resource="http://www.w3.org/2006/time#ProperInterval"/>
        <rdfs:range rdf:resource="http://www.w3.org/2006/time#ProperInterval"/>
        <rdfs:comment xml:lang="es">Asume una direcci�n en el tiempo. Si una entidad temporal T1 est� despu�s de otra entidad temporal T2, entonces el principio de T1 est� despu�s del final de T2.</rdfs:comment>
        <rdfs:comment xml:lang="en">If a proper interval T1 is intervalOverlaps another proper interval T2, then the beginning of T1 is before the beginning of T2, the end of T1 is after the beginning of T2, and the end of T1 is before the end of T2.</rdfs:comment>
        <rdfs:comment xml:lang="es">Si un intervalo propio T1 se solapa con otro intervalo propio T2, entonces el principio de T1 es anterior al principio de T2, el final de T1 es posterior al principio de T2, y el final de T1 es anterior al final de T2.</rdfs:comment>
        <rdfs:label xml:lang="en">interval overlaps</rdfs:label>
        <rdfs:label xml:lang="es">intervalo se solapa</rdfs:label>
        <skos:definition xml:lang="en">If a proper interval T1 is intervalOverlaps another proper interval T2, then the beginning of T1 is before the beginning of T2, the end of T1 is after the beginning of T2, and the end of T1 is before the end of T2.</skos:definition>
        <skos:definition xml:lang="es">Si un intervalo propio T1 se solapa con otro intervalo propio T2, entonces el principio de T1 es anterior al principio de T2, el final de T1 es posterior al principio de T2, y el final de T1 es anterior al final de T2.</skos:definition>
    </owl:ObjectProperty>
    


    <!-- http://www.w3.org/2006/time#intervalStartedBy -->

    <owl:ObjectProperty rdf:about="http://www.w3.org/2006/time#intervalStartedBy">
        <owl:inverseOf rdf:resource="http://www.w3.org/2006/time#intervalStarts"/>
        <rdfs:domain rdf:resource="http://www.w3.org/2006/time#ProperInterval"/>
        <rdfs:range rdf:resource="http://www.w3.org/2006/time#ProperInterval"/>
        <rdfs:comment xml:lang="en">If a proper interval T1 is intervalStarted another proper interval T2, then the beginning of T1 is coincident with the beginning of T2, and the end of T1 is after the end of T2.</rdfs:comment>
        <rdfs:comment xml:lang="es">Si un intervalo propio T1 es empezado por otro intervalo propio T2, entonces el principio de T1 coincide con el principio de T2, y el final de T1 es posterior al final de T2.</rdfs:comment>
        <rdfs:label xml:lang="en">interval started by</rdfs:label>
        <skos:definition xml:lang="en">If a proper interval T1 is intervalStarted another proper interval T2, then the beginning of T1 is coincident with the beginning of T2, and the end of T1 is after the end of T2.</skos:definition>
        <skos:definition xml:lang="es">Si un intervalo propio T1 es empezado por otro intervalo propio T2, entonces el principio de T1 coincide con el principio de T2, y el final de T1 es posterior al final de T2.</skos:definition>
    </owl:ObjectProperty>
    


    <!-- http://www.w3.org/2006/time#intervalStarts -->

    <owl:ObjectProperty rdf:about="http://www.w3.org/2006/time#intervalStarts">
        <rdfs:subPropertyOf rdf:resource="http://www.w3.org/2006/time#intervalIn"/>
        <rdfs:domain rdf:resource="http://www.w3.org/2006/time#ProperInterval"/>
        <rdfs:range rdf:resource="http://www.w3.org/2006/time#ProperInterval"/>
        <rdfs:comment xml:lang="en">If a proper interval T1 is intervalStarts another proper interval T2, then the beginning of T1 is coincident with the beginning of T2, and the end of T1 is before the end of T2.</rdfs:comment>
        <rdfs:comment xml:lang="es">Si un intervalo propio T1 empieza otro intervalo propio T2, entonces del principio de T1 con el principio de T2, y el final de T1 es anterior al final de T2.</rdfs:comment>
        <rdfs:label xml:lang="en">interval starts</rdfs:label>
        <rdfs:label xml:lang="es">intervalo empieza</rdfs:label>
        <skos:definition xml:lang="en">If a proper interval T1 is intervalStarts another proper interval T2, then the beginning of T1 is coincident with the beginning of T2, and the end of T1 is before the end of T2.</skos:definition>
        <skos:definition xml:lang="es">Si un intervalo propio T1 empieza otro intervalo propio T2, entonces del principio de T1 con el final de T2, y el final de T1 es anterior al final de T2.</skos:definition>
    </owl:ObjectProperty>
    


    <!-- http://www.w3.org/2006/time#monthOfYear -->

    <owl:ObjectProperty rdf:about="http://www.w3.org/2006/time#monthOfYear">
        <rdfs:domain rdf:resource="http://www.w3.org/2006/time#GeneralDateTimeDescription"/>
        <rdfs:range rdf:resource="http://www.w3.org/2006/time#MonthOfYear"/>
        <rdfs:comment xml:lang="es">El mes del a�o, cuyo valor es un miembro de la clase &apos;mes del a�o&apos;.</rdfs:comment>
        <rdfs:comment xml:lang="en">The month of the year, whose value is a member of the class time:MonthOfYear</rdfs:comment>
        <rdfs:label xml:lang="es">mes del a�o</rdfs:label>
        <rdfs:label xml:lang="en">month of year</rdfs:label>
        <skos:definition xml:lang="es">El mes del a�o, cuyo valor es un miembro de la clase &apos;mes del a�o&apos;.</skos:definition>
        <skos:definition xml:lang="en">The month of the year, whose value is a member of the class time:MonthOfYear</skos:definition>
        <skos:editorialNote xml:lang="es">Caracter�stica arriesgada - a�adida en la revisi�n de 2017, y todav�a no ampliamente utilizada.</skos:editorialNote>
        <skos:editorialNote xml:lang="en">Feature at risk - added in 2017 revision, and not yet widely used. </skos:editorialNote>
    </owl:ObjectProperty>
    


    <!-- http://www.w3.org/2006/time#timeZone -->

    <owl:ObjectProperty rdf:about="http://www.w3.org/2006/time#timeZone">
        <rdfs:domain rdf:resource="http://www.w3.org/2006/time#GeneralDateTimeDescription"/>
        <rdfs:range rdf:resource="http://www.w3.org/2006/time#TimeZone"/>
        <rdfs:comment xml:lang="en">The time zone for clock elements in the temporal position</rdfs:comment>
        <rdfs:label xml:lang="es">en huso horario</rdfs:label>
        <rdfs:label xml:lang="en">in time zone</rdfs:label>
        <skos:historyNote xml:lang="es">En la versi�n original de OWL-Time de 2006, el rango de &apos;en huso horario&apos; se defini� en un espacio de nombres diferente &quot;http://www.w3.org/2006/timezone#&quot;.
            Un axioma de alineaci�n permite que los datos codificados de acuerdo con la versi�n anterior sean consistentes con la ontolog�a actualizada.</skos:historyNote>
        <skos:historyNote>In the original 2006 version of OWL-Time, the range of time:timeZone was a TimeZone class in a separate namespace &quot;http://www.w3.org/2006/timezone#&quot;. 
An alignment axiom 
	tzont:TimeZone rdfs:subClassOf time:TimeZone . 
allows data encoded according to the previous version to be consistent with the updated ontology. </skos:historyNote>
        <skos:note>IANA maintains a database of timezones. These are well maintained and generally considered authoritative, but individual items are not available at individual URIs, so cannot be used directly in data expressed using OWL-Time.

DBPedia provides a set of resources corresponding to the IANA timezones, with a URI for each (e.g. http://dbpedia.org/resource/Australia/Eucla). The World Clock service also provides a list of time zones with the description of each available as an individual webpage with a convenient individual URI (e.g. https://www.timeanddate.com/time/zones/acwst). These or other, similar, resources might be used as a value of the time:timeZone property.</skos:note>
        <skos:note xml:lang="es">IANA mantiene una base de datos de husos horarios. �stas est�n bien mantenidas y generalmente se consideran autorizadas, pero los �tems individuales no est�n disponibles en URIs individuales, por tanto, no se pueden utilizar directamente en datos expresados utilizando OWL-Time.
            La BDPedia proporciona un conjunto de recursos correspondientes a los husos horarios de IANA, con una URI para cada uno (por ejemplo, http://dbpedia.org/resource/Australia/Eucla). El Servicio de Reloj Mundial tambi�n proporciona una lista de husos horarios con la descripci�n de cada uno de los disponibles como una p�gina Web individual con una URI adecuada individual (por ejemplo, https://www.timeanddate.com/time/zones/acwst). �stos, y otros recursos similares, se puden usar como un valor de la propiedad &apos;huso horario&apos;.</skos:note>
    </owl:ObjectProperty>
    


    <!-- http://www.w3.org/2006/time#unitType -->

    <owl:ObjectProperty rdf:about="http://www.w3.org/2006/time#unitType">
        <rdfs:domain>
            <owl:Class>
                <owl:unionOf rdf:parseType="Collection">
                    <rdf:Description rdf:about="http://www.w3.org/2006/time#Duration"/>
                    <rdf:Description rdf:about="http://www.w3.org/2006/time#GeneralDateTimeDescription"/>
                </owl:unionOf>
            </owl:Class>
        </rdfs:domain>
        <rdfs:range rdf:resource="http://www.w3.org/2006/time#TemporalUnit"/>
        <rdfs:comment xml:lang="es">La unidad de tiempo que proporciona la precisi�n de un valor fecha-hora o la escala de una extensi�n temporal.</rdfs:comment>
        <rdfs:comment xml:lang="en">The temporal unit which provides the precision of a date-time value or scale of a temporal extent</rdfs:comment>
        <rdfs:label xml:lang="en">temporal unit type</rdfs:label>
        <rdfs:label xml:lang="es">tipo de unidad temporal</rdfs:label>
    </owl:ObjectProperty>
    


    <!-- 
    ///////////////////////////////////////////////////////////////////////////////////////
    //
    // Data properties
    //
    ///////////////////////////////////////////////////////////////////////////////////////
     -->

    


    <!-- http://www.w3.org/2006/time#day -->

    <owl:DatatypeProperty rdf:about="http://www.w3.org/2006/time#day">
        <rdfs:domain rdf:resource="http://www.w3.org/2006/time#GeneralDateTimeDescription"/>
        <rdfs:comment xml:lang="en">Day position in a calendar-clock system.

The range of this property is not specified, so can be replaced by any specific representation of a calendar day from any calendar. </rdfs:comment>
        <rdfs:comment xml:lang="es">Posici�n de d�a en un sistema calendario-reloj.</rdfs:comment>
        <rdfs:label xml:lang="en">day</rdfs:label>
        <rdfs:label xml:lang="es">d�a</rdfs:label>
        <skos:definition xml:lang="en">Day position in a calendar-clock system.

The range of this property is not specified, so can be replaced by any specific representation of a calendar day from any calendar. </skos:definition>
        <skos:definition xml:lang="es">Posici�n de d�a en un sistema calendario-reloj.

El rango de esta propiedad no est� especificado, por tanto, se puede reemplazar por una representaci�n espec�fica de un d�a de calendario de cualquier calendario.</skos:definition>
    </owl:DatatypeProperty>
    


    <!-- http://www.w3.org/2006/time#dayOfYear -->

    <owl:DatatypeProperty rdf:about="http://www.w3.org/2006/time#dayOfYear">
        <rdfs:domain rdf:resource="http://www.w3.org/2006/time#GeneralDateTimeDescription"/>
        <rdfs:range rdf:resource="http://www.w3.org/2001/XMLSchema#nonNegativeInteger"/>
        <rdfs:comment xml:lang="es">El n�mero de d�a en el a�o.</rdfs:comment>
        <rdfs:comment xml:lang="en">The number of the day within the year</rdfs:comment>
        <rdfs:label xml:lang="en">day of year</rdfs:label>
        <rdfs:label xml:lang="es">d�a del a�o</rdfs:label>
        <skos:definition xml:lang="es">El n�mero de d�a en el a�o.</skos:definition>
        <skos:definition xml:lang="en">The number of the day within the year</skos:definition>
    </owl:DatatypeProperty>
    


    <!-- http://www.w3.org/2006/time#days -->

    <owl:DatatypeProperty rdf:about="http://www.w3.org/2006/time#days">
        <rdfs:domain rdf:resource="http://www.w3.org/2006/time#GeneralDurationDescription"/>
        <rdfs:range rdf:resource="http://www.w3.org/2001/XMLSchema#decimal"/>
        <rdfs:comment xml:lang="es">Longitud de, o elemento de la longitud de, una extensi�n temporal expresada en d�as.</rdfs:comment>
        <rdfs:comment xml:lang="en">length of, or element of the length of, a temporal extent expressed in days</rdfs:comment>
        <rdfs:label xml:lang="en">days duration</rdfs:label>
        <rdfs:label xml:lang="es">duraci�n en d�as</rdfs:label>
        <skos:definition xml:lang="es">Longitud de, o elemento de la longitud de, una extensi�n temporal expresada en d�as.</skos:definition>
        <skos:definition xml:lang="en">length of, or element of the length of, a temporal extent expressed in days</skos:definition>
    </owl:DatatypeProperty>
    


    <!-- http://www.w3.org/2006/time#hasXSDDuration -->

    <owl:DatatypeProperty rdf:about="http://www.w3.org/2006/time#hasXSDDuration">
        <rdfs:domain rdf:resource="http://www.w3.org/2006/time#TemporalEntity"/>
        <rdfs:range rdf:resource="http://www.w3.org/2001/XMLSchema#duration"/>
        <rdfs:comment xml:lang="es">Extensi�n de una entidad temporal, expresada utilizando xsd:duration.</rdfs:comment>
        <rdfs:comment xml:lang="en">Extent of a temporal entity, expressed using xsd:duration</rdfs:comment>
        <rdfs:label xml:lang="en">has XSD duration</rdfs:label>
        <rdfs:label xml:lang="es">tiene duraci�n XSD</rdfs:label>
        <skos:definition xml:lang="es">Extensi�n de una entidad temporal, expresada utilizando xsd:duration.</skos:definition>
        <skos:definition xml:lang="en">Extent of a temporal entity, expressed using xsd:duration</skos:definition>
        <skos:editorialNote xml:lang="es">Caracter�stica arriesgada - a�adida en la revisi�n de 2017, y todav�a no ampliamente utilizada.</skos:editorialNote>
        <skos:editorialNote xml:lang="en">Feature at risk - added in 2017 revision, and not yet widely used. </skos:editorialNote>
    </owl:DatatypeProperty>
    


    <!-- http://www.w3.org/2006/time#hour -->

    <owl:DatatypeProperty rdf:about="http://www.w3.org/2006/time#hour">
        <rdfs:domain rdf:resource="http://www.w3.org/2006/time#GeneralDateTimeDescription"/>
        <rdfs:range rdf:resource="http://www.w3.org/2001/XMLSchema#nonNegativeInteger"/>
        <rdfs:comment xml:lang="en">Hour position in a calendar-clock system.</rdfs:comment>
        <rdfs:comment xml:lang="es">Posici�n de hora en un sistema calendario-reloj.</rdfs:comment>
        <rdfs:label xml:lang="es">hora</rdfs:label>
        <rdfs:label xml:lang="en">hour</rdfs:label>
        <skos:definition xml:lang="en">Hour position in a calendar-clock system.</skos:definition>
        <skos:definition xml:lang="es">Posici�n de hora en un sistema calendario-reloj.</skos:definition>
    </owl:DatatypeProperty>
    


    <!-- http://www.w3.org/2006/time#hours -->

    <owl:DatatypeProperty rdf:about="http://www.w3.org/2006/time#hours">
        <rdfs:domain rdf:resource="http://www.w3.org/2006/time#GeneralDurationDescription"/>
        <rdfs:range rdf:resource="http://www.w3.org/2001/XMLSchema#decimal"/>
        <rdfs:comment xml:lang="es">Longitud de, o elemento de la longitud de, una extensi�n temporal expresada en horas.</rdfs:comment>
        <rdfs:comment xml:lang="en">length of, or element of the length of, a temporal extent expressed in hours</rdfs:comment>
        <rdfs:label xml:lang="es">duraci�n en horas</rdfs:label>
        <rdfs:label xml:lang="en">hours duration</rdfs:label>
        <skos:definition xml:lang="es">Longitud de, o elemento de la longitud de, una extensi�n temporal expresada en horas.</skos:definition>
        <skos:definition xml:lang="en">length of, or element of the length of, a temporal extent expressed in hours</skos:definition>
    </owl:DatatypeProperty>
    


    <!-- http://www.w3.org/2006/time#inXSDDate -->

    <owl:DatatypeProperty rdf:about="http://www.w3.org/2006/time#inXSDDate">
        <rdfs:domain rdf:resource="http://www.w3.org/2006/time#Instant"/>
        <rdfs:range rdf:resource="http://www.w3.org/2001/XMLSchema#date"/>
        <rdfs:comment xml:lang="es">Posici�n de un instante, expresado utilizando xsd:date.</rdfs:comment>
        <rdfs:comment xml:lang="en">Position of an instant, expressed using xsd:date</rdfs:comment>
        <rdfs:label xml:lang="es">en fecha XSD</rdfs:label>
        <rdfs:label xml:lang="en">in XSD date</rdfs:label>
        <skos:definition xml:lang="es">Posici�n de un instante, expresado utilizando xsd:date.</skos:definition>
        <skos:definition xml:lang="en">Position of an instant, expressed using xsd:date</skos:definition>
    </owl:DatatypeProperty>
    


    <!-- http://www.w3.org/2006/time#inXSDDateTime -->

    <owl:DatatypeProperty rdf:about="http://www.w3.org/2006/time#inXSDDateTime">
        <rdfs:domain rdf:resource="http://www.w3.org/2006/time#Instant"/>
        <rdfs:range rdf:resource="http://www.w3.org/2001/XMLSchema#dateTime"/>
        <rdfs:comment xml:lang="es">Posici�n de un instante, expresado utilizando xsd:dateTime.</rdfs:comment>
        <rdfs:comment xml:lang="en">Position of an instant, expressed using xsd:dateTime</rdfs:comment>
        <rdfs:label xml:lang="es">en fecha-tiempo XSD</rdfs:label>
        <rdfs:label xml:lang="en">in XSD Date-Time</rdfs:label>
        <owl:deprecated rdf:datatype="http://www.w3.org/2001/XMLSchema#boolean">true</owl:deprecated>
        <skos:definition xml:lang="es">Posici�n de un instante, expresado utilizando xsd:dateTime.</skos:definition>
        <skos:definition xml:lang="en">Position of an instant, expressed using xsd:dateTime</skos:definition>
        <skos:note xml:lang="es">La propiedad &apos;en fecha-hora XSD&apos; ha sido reemplazada por &apos;en fecha-sello de tiempo XSD&apos; que hace obligatorio el campo &apos;huso horario&apos;.</skos:note>
        <skos:note xml:lang="en">The property :inXSDDateTime is replaced by :inXSDDateTimeStamp which makes the time-zone field mandatory.</skos:note>
    </owl:DatatypeProperty>
    


    <!-- http://www.w3.org/2006/time#inXSDDateTimeStamp -->

    <owl:DatatypeProperty rdf:about="http://www.w3.org/2006/time#inXSDDateTimeStamp">
        <rdfs:domain rdf:resource="http://www.w3.org/2006/time#Instant"/>
        <rdfs:range rdf:resource="http://www.w3.org/2001/XMLSchema#dateTimeStamp"/>
        <rdfs:comment xml:lang="es">Posici�n de un instante, expresado utilizando xsd:dateTimeStamp.</rdfs:comment>
        <rdfs:comment xml:lang="en">Position of an instant, expressed using xsd:dateTimeStamp</rdfs:comment>
        <rdfs:label xml:lang="es">en fecha-sello de tiempo XSD</rdfs:label>
        <rdfs:label xml:lang="en">in XSD Date-Time-Stamp</rdfs:label>
        <skos:definition xml:lang="es">Posici�n de un instante, expresado utilizando xsd:dateTimeStamp.</skos:definition>
        <skos:definition xml:lang="en">Position of an instant, expressed using xsd:dateTimeStamp</skos:definition>
    </owl:DatatypeProperty>
    


    <!-- http://www.w3.org/2006/time#inXSDgYear -->

    <owl:DatatypeProperty rdf:about="http://www.w3.org/2006/time#inXSDgYear">
        <rdfs:domain rdf:resource="http://www.w3.org/2006/time#Instant"/>
        <rdfs:range rdf:resource="http://www.w3.org/2001/XMLSchema#gYear"/>
        <rdfs:comment xml:lang="es">Posici�n de un instante, expresado utilizando xsd:gYear.</rdfs:comment>
        <rdfs:comment xml:lang="en">Position of an instant, expressed using xsd:gYear</rdfs:comment>
        <rdfs:label xml:lang="es">en a�o gregoriano XSD</rdfs:label>
        <rdfs:label xml:lang="en">in XSD g-Year</rdfs:label>
        <skos:definition xml:lang="es">Posici�n de un instante, expresado utilizando xsd:gYear.</skos:definition>
        <skos:definition xml:lang="en">Position of an instant, expressed using xsd:gYear</skos:definition>
    </owl:DatatypeProperty>
    


    <!-- http://www.w3.org/2006/time#inXSDgYearMonth -->

    <owl:DatatypeProperty rdf:about="http://www.w3.org/2006/time#inXSDgYearMonth">
        <rdfs:domain rdf:resource="http://www.w3.org/2006/time#Instant"/>
        <rdfs:range rdf:resource="http://www.w3.org/2001/XMLSchema#gYearMonth"/>
        <rdfs:comment xml:lang="es">Posici�n de un instante, expresado utilizando xsd:gYearMonth.</rdfs:comment>
        <rdfs:comment xml:lang="en">Position of an instant, expressed using xsd:gYearMonth</rdfs:comment>
        <rdfs:label xml:lang="es">en a�o-mes gregoriano XSD</rdfs:label>
        <rdfs:label xml:lang="en">in XSD g-YearMonth</rdfs:label>
        <skos:definition xml:lang="es">Posici�n de un instante, expresado utilizando xsd:gYearMonth.</skos:definition>
        <skos:definition xml:lang="en">Position of an instant, expressed using xsd:gYearMonth</skos:definition>
    </owl:DatatypeProperty>
    


    <!-- http://www.w3.org/2006/time#minute -->

    <owl:DatatypeProperty rdf:about="http://www.w3.org/2006/time#minute">
        <rdfs:domain rdf:resource="http://www.w3.org/2006/time#GeneralDateTimeDescription"/>
        <rdfs:range rdf:resource="http://www.w3.org/2001/XMLSchema#nonNegativeInteger"/>
        <rdfs:comment xml:lang="en">Minute position in a calendar-clock system.</rdfs:comment>
        <rdfs:comment xml:lang="es">Posici�n de minuto en un sistema calendario-reloj.</rdfs:comment>
        <rdfs:label xml:lang="en">minute</rdfs:label>
        <rdfs:label xml:lang="es">minuto</rdfs:label>
        <skos:definition xml:lang="en">Minute position in a calendar-clock system.</skos:definition>
        <skos:definition xml:lang="es">Posici�n de minuto en un sistema calendario-reloj.</skos:definition>
    </owl:DatatypeProperty>
    


    <!-- http://www.w3.org/2006/time#minutes -->

    <owl:DatatypeProperty rdf:about="http://www.w3.org/2006/time#minutes">
        <rdfs:domain rdf:resource="http://www.w3.org/2006/time#GeneralDurationDescription"/>
        <rdfs:range rdf:resource="http://www.w3.org/2001/XMLSchema#decimal"/>
        <rdfs:comment xml:lang="es">Longitud de, o elemento de la longitud de, una extensi�n temporal expresada en minutos.</rdfs:comment>
        <rdfs:comment xml:lang="en">length, or element of, a temporal extent expressed in minutes</rdfs:comment>
        <rdfs:label xml:lang="en">minutes</rdfs:label>
        <rdfs:label xml:lang="es">minutos</rdfs:label>
        <skos:definition xml:lang="es">Longitud de, o elemento de la longitud de, una extensi�n temporal expresada en minutos.</skos:definition>
        <skos:definition xml:lang="en">length, or element of, a temporal extent expressed in minutes</skos:definition>
    </owl:DatatypeProperty>
    


    <!-- http://www.w3.org/2006/time#month -->

    <owl:DatatypeProperty rdf:about="http://www.w3.org/2006/time#month">
        <rdfs:domain rdf:resource="http://www.w3.org/2006/time#GeneralDateTimeDescription"/>
        <rdfs:comment xml:lang="en">Month position in a calendar-clock system.

The range of this property is not specified, so can be replaced by any specific representation of a calendar month from any calendar. </rdfs:comment>
        <rdfs:comment xml:lang="es">Posici�n de mes en un sistema calendario-reloj.
    El rango de esta propiedad no est� especificado, por tanto, se puede reemplazar por cualquier representaci�n espec�fica de un mes de calendario de un calendario cualquiera.</rdfs:comment>
        <rdfs:label xml:lang="es">mes</rdfs:label>
        <rdfs:label xml:lang="en">month</rdfs:label>
        <skos:definition xml:lang="en">Month position in a calendar-clock system.

The range of this property is not specified, so can be replaced by any specific representation of a calendar month from any calendar. </skos:definition>
        <skos:definition xml:lang="es">Posici�n de mes en un sistema calendario-reloj.
            El rango de esta propiedad no est� especificado, por tanto, se puede reemplazar por cualquier representaci�n espec�fica de un mes de calendario de un calendario cualquiera.</skos:definition>
    </owl:DatatypeProperty>
    


    <!-- http://www.w3.org/2006/time#months -->

    <owl:DatatypeProperty rdf:about="http://www.w3.org/2006/time#months">
        <rdfs:domain rdf:resource="http://www.w3.org/2006/time#GeneralDurationDescription"/>
        <rdfs:range rdf:resource="http://www.w3.org/2001/XMLSchema#decimal"/>
        <rdfs:comment xml:lang="es">Longitud de, o elemento de la longitud de, una extensi�n temporal expresada en meses.</rdfs:comment>
        <rdfs:comment xml:lang="en">length of, or element of the length of, a temporal extent expressed in months</rdfs:comment>
        <rdfs:label xml:lang="es">duraci�n en meses</rdfs:label>
        <rdfs:label xml:lang="en">months duration</rdfs:label>
        <skos:definition xml:lang="es">Longitud de, o elemento de la longitud de, una extensi�n temporal expresada en meses.</skos:definition>
        <skos:definition xml:lang="en">length of, or element of the length of, a temporal extent expressed in months</skos:definition>
    </owl:DatatypeProperty>
    


    <!-- http://www.w3.org/2006/time#nominalPosition -->

    <owl:DatatypeProperty rdf:about="http://www.w3.org/2006/time#nominalPosition">
        <rdfs:domain rdf:resource="http://www.w3.org/2006/time#TimePosition"/>
        <rdfs:range rdf:resource="http://www.w3.org/2001/XMLSchema#string"/>
        <rdfs:comment xml:lang="es">El valor (nominal) que indica posici�n temporal en un sistema de referencia ordinal.</rdfs:comment>
        <rdfs:comment xml:lang="en">The (nominal) value indicating temporal position in an ordinal reference system </rdfs:comment>
        <rdfs:label xml:lang="en">Name of temporal position</rdfs:label>
        <rdfs:label xml:lang="es">nombre de posici�n temporal</rdfs:label>
        <skos:definition xml:lang="es">El valor (nominal) que indica posici�n temporal en un sistema de referencia ordinal.</skos:definition>
        <skos:definition xml:lang="en">The (nominal) value indicating temporal position in an ordinal reference system </skos:definition>
    </owl:DatatypeProperty>
    


    <!-- http://www.w3.org/2006/time#numericDuration -->

    <owl:DatatypeProperty rdf:about="http://www.w3.org/2006/time#numericDuration">
        <rdfs:domain rdf:resource="http://www.w3.org/2006/time#Duration"/>
        <rdfs:range rdf:resource="http://www.w3.org/2001/XMLSchema#decimal"/>
        <rdfs:comment xml:lang="es">Valor de una extensi�n temporal expresada como un n�mero decimal escalado por una unidad de tiempo.</rdfs:comment>
        <rdfs:comment xml:lang="en">Value of a temporal extent expressed as a decimal number scaled by a temporal unit</rdfs:comment>
        <rdfs:label xml:lang="en">Numeric value of temporal duration</rdfs:label>
        <rdfs:label xml:lang="es">valor num�rico de duraci�n temporal</rdfs:label>
        <skos:definition xml:lang="es">Valor de una extensi�n temporal expresada como un n�mero decimal escalado por una unidad de tiempo.</skos:definition>
        <skos:definition xml:lang="en">Value of a temporal extent expressed as a decimal number scaled by a temporal unit</skos:definition>
    </owl:DatatypeProperty>
    


    <!-- http://www.w3.org/2006/time#numericPosition -->

    <owl:DatatypeProperty rdf:about="http://www.w3.org/2006/time#numericPosition">
        <rdfs:domain rdf:resource="http://www.w3.org/2006/time#TimePosition"/>
        <rdfs:range rdf:resource="http://www.w3.org/2001/XMLSchema#decimal"/>
        <rdfs:comment xml:lang="es">El valor (num�rico) que indica posici�n temporal en un sistema de referencia ordinal.</rdfs:comment>
        <rdfs:comment xml:lang="en">The (numeric) value indicating position within a temporal coordinate system </rdfs:comment>
        <rdfs:label xml:lang="en">Numeric value of temporal position</rdfs:label>
        <rdfs:label xml:lang="es">valor num�rico de posici�n temporal</rdfs:label>
        <skos:definition xml:lang="es">El valor (num�rico) que indica posici�n temporal en un sistema de referencia ordinal.</skos:definition>
        <skos:definition xml:lang="en">The (numeric) value indicating position within a temporal coordinate system </skos:definition>
    </owl:DatatypeProperty>
    


    <!-- http://www.w3.org/2006/time#second -->

    <owl:DatatypeProperty rdf:about="http://www.w3.org/2006/time#second">
        <rdfs:domain rdf:resource="http://www.w3.org/2006/time#GeneralDateTimeDescription"/>
        <rdfs:range rdf:resource="http://www.w3.org/2001/XMLSchema#decimal"/>
        <rdfs:comment xml:lang="es">Posici�n de segundo en un sistema calendario-reloj.</rdfs:comment>
        <rdfs:comment xml:lang="en">Second position in a calendar-clock system.</rdfs:comment>
        <rdfs:label xml:lang="en">second</rdfs:label>
        <rdfs:label xml:lang="es">segundo</rdfs:label>
    </owl:DatatypeProperty>
    


    <!-- http://www.w3.org/2006/time#seconds -->

    <owl:DatatypeProperty rdf:about="http://www.w3.org/2006/time#seconds">
        <rdfs:domain rdf:resource="http://www.w3.org/2006/time#GeneralDurationDescription"/>
        <rdfs:range rdf:resource="http://www.w3.org/2001/XMLSchema#decimal"/>
        <rdfs:comment xml:lang="es">Longitud de, o elemento de la longitud de, una extensi�n temporal expresada en segundos.</rdfs:comment>
        <rdfs:comment xml:lang="en">length of, or element of the length of, a temporal extent expressed in seconds</rdfs:comment>
        <rdfs:label xml:lang="es">duraci�n en segundos</rdfs:label>
        <rdfs:label xml:lang="en">seconds duration</rdfs:label>
        <rdfs:seeAlso rdf:resource="http://www.bipm.org/en/publications/si-brochure/second.html"/>
    </owl:DatatypeProperty>
    


    <!-- http://www.w3.org/2006/time#week -->

    <owl:DatatypeProperty rdf:about="http://www.w3.org/2006/time#week">
        <rdfs:domain rdf:resource="http://www.w3.org/2006/time#GeneralDateTimeDescription"/>
        <rdfs:range rdf:resource="http://www.w3.org/2001/XMLSchema#nonNegativeInteger"/>
        <rdfs:comment xml:lang="es">N�mero de semana en el a�o.</rdfs:comment>
        <rdfs:comment xml:lang="en">Week number within the year.</rdfs:comment>
        <rdfs:label xml:lang="es">semana</rdfs:label>
        <rdfs:label xml:lang="en">week</rdfs:label>
        <skos:note xml:lang="en">Weeks are numbered differently depending on the calendar in use and the local language or cultural conventions (locale). ISO-8601 specifies that the first week of the year includes at least four days, and that Monday is the first day of the week. In that system, week 1 is the week that contains the first Thursday in the year.</skos:note>
        <skos:scopeNote xml:lang="es">Las semanas est�n numeradas de forma diferente dependiendo del calendario en uso y de las convenciones ling��sticas y culturales locales (locale en ingl�s). El ISO-8601 especifica que la primera semana del a�o incluye al menos cuatro d�as, y que el lunes es el primer d�a de la semana. En ese sistema, la semana 1 es la semana que contiene el primer jueves del a�o.</skos:scopeNote>
    </owl:DatatypeProperty>
    


    <!-- http://www.w3.org/2006/time#weeks -->

    <owl:DatatypeProperty rdf:about="http://www.w3.org/2006/time#weeks">
        <rdfs:domain rdf:resource="http://www.w3.org/2006/time#GeneralDurationDescription"/>
        <rdfs:range rdf:resource="http://www.w3.org/2001/XMLSchema#decimal"/>
        <rdfs:comment xml:lang="es">Longitud de, o elemento de la longitud de, una extensi�n temporal expresada en semanas.</rdfs:comment>
        <rdfs:comment xml:lang="en">length of, or element of the length of, a temporal extent expressed in weeks</rdfs:comment>
        <rdfs:label xml:lang="es">duraci�n en semanas</rdfs:label>
        <rdfs:label xml:lang="en">weeks duration</rdfs:label>
    </owl:DatatypeProperty>
    


    <!-- http://www.w3.org/2006/time#xsdDateTime -->

    <owl:DatatypeProperty rdf:about="http://www.w3.org/2006/time#xsdDateTime">
        <rdfs:domain rdf:resource="http://www.w3.org/2006/time#DateTimeInterval"/>
        <rdfs:range rdf:resource="http://www.w3.org/2001/XMLSchema#dateTime"/>
        <rdfs:comment xml:lang="es">Valor de &apos;intervalo de fecha-hora&apos; expresado como un valor compacto.</rdfs:comment>
        <rdfs:comment xml:lang="en">Value of DateTimeInterval expressed as a compact value.</rdfs:comment>
        <rdfs:label xml:lang="en">has XSD date-time</rdfs:label>
        <rdfs:label xml:lang="es">tiene fecha-hora XSD</rdfs:label>
        <owl:deprecated rdf:datatype="http://www.w3.org/2001/XMLSchema#boolean">true</owl:deprecated>
        <skos:note xml:lang="en">Using xsd:dateTime in this place means that the duration of the interval is implicit: it corresponds to the length of the smallest non-zero element of the date-time literal. However, this rule cannot be used for intervals whose duration is more than one rank smaller than the starting time - e.g. the first minute or second of a day, the first hour of a month, or the first day of a year. In these cases the desired interval cannot be distinguished from the interval corresponding to the next rank up. Because of this essential ambiguity, use of this property is not recommended and it is deprecated.</skos:note>
        <skos:note>Utilizando xsd:dateTime en este lugar significa que la duraci�n del intervalo est� impl�cita: se corresponde con la longitud del elemento m�s peque�o distinto de cero del literal fecha-hora. Sin embargo, esta regla no se puede utilizar para intervalos cuya duraci�n es mayor que un rango m�s peque�o que el tiempo de comienzo - p.ej. el primer minuto o segundo del d�a, la primera hora del mes, o el primer d�a del a�o. En estos casos el intervalo deseado no se puede distinguir del intervalo correspondiente al pr�ximo rango m�s alto. Debido a esta ambig�edad esencial, no se recomienda el uso de esta propiedad y est� desaprobada.</skos:note>
    </owl:DatatypeProperty>
    


    <!-- http://www.w3.org/2006/time#year -->

    <owl:DatatypeProperty rdf:about="http://www.w3.org/2006/time#year">
        <rdfs:domain rdf:resource="http://www.w3.org/2006/time#GeneralDateTimeDescription"/>
        <rdfs:comment xml:lang="es">Posici�n de a�o en un sistema calendario-reloj.

l rango de esta propiedad no est� especificado, por tanto, se puede reemplazar por cualquier representaci�n espec�fica de un a�o de calendario de un calendario cualquiera.</rdfs:comment>
        <rdfs:comment xml:lang="en">Year position in a calendar-clock system.

The range of this property is not specified, so can be replaced by any specific representation of a calendar year from any calendar. </rdfs:comment>
        <rdfs:label xml:lang="en">year</rdfs:label>
    </owl:DatatypeProperty>
    


    <!-- http://www.w3.org/2006/time#years -->

    <owl:DatatypeProperty rdf:about="http://www.w3.org/2006/time#years">
        <rdfs:domain rdf:resource="http://www.w3.org/2006/time#GeneralDurationDescription"/>
        <rdfs:range rdf:resource="http://www.w3.org/2001/XMLSchema#decimal"/>
        <rdfs:comment xml:lang="es">Longitud de, o elemento de la longitud de, una extensi�n temporal expresada en a�os.</rdfs:comment>
        <rdfs:comment xml:lang="en">length of, or element of the length of, a temporal extent expressed in years</rdfs:comment>
        <rdfs:label xml:lang="es">duraci�n en a�os</rdfs:label>
        <rdfs:label xml:lang="en">years duration</rdfs:label>
    </owl:DatatypeProperty>
    


    <!-- 
    ///////////////////////////////////////////////////////////////////////////////////////
    //
    // Classes
    //
    ///////////////////////////////////////////////////////////////////////////////////////
     -->

    


    <!-- http://www.w3.org/2006/time#DateTimeDescription -->

    <owl:Class rdf:about="http://www.w3.org/2006/time#DateTimeDescription">
        <rdfs:subClassOf rdf:resource="http://www.w3.org/2006/time#GeneralDateTimeDescription"/>
        <rdfs:subClassOf>
            <owl:Restriction>
                <owl:onProperty rdf:resource="http://www.w3.org/2006/time#hasTRS"/>
                <owl:hasValue rdf:resource="http://www.opengis.net/def/uom/ISO-8601/0/Gregorian"/>
            </owl:Restriction>
        </rdfs:subClassOf>
        <rdfs:subClassOf>
            <owl:Restriction>
                <owl:onProperty rdf:resource="http://www.w3.org/2006/time#day"/>
                <owl:allValuesFrom rdf:resource="http://www.w3.org/2001/XMLSchema#gDay"/>
            </owl:Restriction>
        </rdfs:subClassOf>
        <rdfs:subClassOf>
            <owl:Restriction>
                <owl:onProperty rdf:resource="http://www.w3.org/2006/time#month"/>
                <owl:allValuesFrom rdf:resource="http://www.w3.org/2001/XMLSchema#gMonth"/>
            </owl:Restriction>
        </rdfs:subClassOf>
        <rdfs:subClassOf>
            <owl:Restriction>
                <owl:onProperty rdf:resource="http://www.w3.org/2006/time#year"/>
                <owl:allValuesFrom rdf:resource="http://www.w3.org/2001/XMLSchema#gYear"/>
            </owl:Restriction>
        </rdfs:subClassOf>
        <rdfs:comment xml:lang="es">Descripci�n de fecha y tiempo estructurada con valores separados para los diferentes elementos de un sistema calendario-reloj. El sistema de referencia temporal est� fijado al calendario gregoriano, y el rango de las propiedades a�o, mes, d�a restringidas a los correspondientes tipos del XML Schema xsd:gYear, xsd:gMonth y xsd:gDay respectivamente.</rdfs:comment>
        <rdfs:comment xml:lang="en">Description of date and time structured with separate values for the various elements of a calendar-clock system. The temporal reference system is fixed to Gregorian Calendar, and the range of year, month, day properties restricted to corresponding XML Schema types xsd:gYear, xsd:gMonth and xsd:gDay, respectively.</rdfs:comment>
        <rdfs:label xml:lang="en">Date-Time description</rdfs:label>
        <rdfs:label xml:lang="es">descripci�n de fecha-tiempo</rdfs:label>
        <skos:definition xml:lang="es">Descripci�n de fecha y tiempo estructurada con valores separados para los diferentes elementos de un sistema calendario-reloj. El sistema de referencia temporal est� fijado al calendario gregoriano, y el rango de las propiedades a�o, mes, d�a restringidas a los correspondientes tipos del XML Schema xsd:gYear, xsd:gMonth y xsd:gDay respectivamente.</skos:definition>
        <skos:definition xml:lang="en">Description of date and time structured with separate values for the various elements of a calendar-clock system. The temporal reference system is fixed to Gregorian Calendar, and the range of year, month, day properties restricted to corresponding XML Schema types xsd:gYear, xsd:gMonth and xsd:gDay, respectively.</skos:definition>
    </owl:Class>
    


    <!-- http://www.w3.org/2006/time#DateTimeInterval -->

    <owl:Class rdf:about="http://www.w3.org/2006/time#DateTimeInterval">
        <rdfs:subClassOf rdf:resource="http://www.w3.org/2006/time#ProperInterval"/>
        <rdfs:comment xml:lang="es">&apos;intervalo de fecha-hora&apos; es una subclase de &apos;intervalo propio&apos;, definida utilizando el multi-elemento &apos;descripci�n de fecha-hora&apos;.</rdfs:comment>
        <rdfs:comment xml:lang="en">DateTimeInterval is a subclass of ProperInterval, defined using the multi-element DateTimeDescription.</rdfs:comment>
        <rdfs:label xml:lang="en">Date-time interval</rdfs:label>
        <rdfs:label xml:lang="es">intervalo de fecha-hora</rdfs:label>
        <skos:definition xml:lang="es">&apos;intervalo de fecha-hora&apos; es una subclase de &apos;intervalo propio&apos;, definida utilizando el multi-elemento &apos;descripci�n de fecha-hora&apos;.</skos:definition>
        <skos:definition xml:lang="en">DateTimeInterval is a subclass of ProperInterval, defined using the multi-element DateTimeDescription.</skos:definition>
        <skos:note xml:lang="es">&apos;intervalo de fecha-hora&apos; se puede utilizar s�lo para un intervalo cuyos l�mites coinciden con un elemento de fecha-hora alineados con el calendario y la zona horaria indicados. Por ejemplo, aunque ambos tienen una duraci�n de un d�a, el intervalo de 24 horas que empieza en la media noche del comienzo del 8 mayo en Europa Central se puede expresar como un &apos;intervalo de fecha-hora&apos;, el intervalo de 24 horas que empieza a las 1:30pm no.</skos:note>
        <skos:note xml:lang="en">:DateTimeInterval can only be used for an interval whose limits coincide with a date-time element aligned to the calendar and timezone indicated. For example, while both have a duration of one day, the 24-hour interval beginning at midnight at the beginning of 8 May in Central Europe can be expressed as a :DateTimeInterval, but the 24-hour interval starting at 1:30pm cannot.</skos:note>
    </owl:Class>
    


    <!-- http://www.w3.org/2006/time#DayOfWeek -->

    <owl:Class rdf:about="http://www.w3.org/2006/time#DayOfWeek">
        <rdfs:subClassOf rdf:resource="http://www.w3.org/2002/07/owl#Thing"/>
        <rdfs:comment xml:lang="es">El d�a de la semana</rdfs:comment>
        <rdfs:comment xml:lang="en">The day of week</rdfs:comment>
        <rdfs:label xml:lang="en">Day of week</rdfs:label>
        <rdfs:label xml:lang="es">d�a de la semana</rdfs:label>
        <skos:changeNote xml:lang="en">Remove enumeration from definition, in order to allow other days to be used when required in other calendars. 
NOTE: existing days are still present as members of the class, but the class membership is now open. 

In the original OWL-Time the following constraint appeared: 
  owl:oneOf (
      time:Monday
      time:Tuesday
      time:Wednesday
      time:Thursday
      time:Friday
      time:Saturday
      time:Sunday
    ) ;</skos:changeNote>
        <skos:definition xml:lang="es">El d�a de la semana</skos:definition>
        <skos:definition xml:lang="en">The day of week</skos:definition>
        <skos:note xml:lang="es">La pertenencia a la clase &apos;d�a de la semana&apos; est� abierta, para permitir longitudes de semana alternativas y diferentes nombres de d�as.</skos:note>
        <skos:note xml:lang="en">Membership of the class :DayOfWeek is open, to allow for alternative week lengths and different day names.</skos:note>
    </owl:Class>
    


    <!-- http://www.w3.org/2006/time#Duration -->

    <owl:Class rdf:about="http://www.w3.org/2006/time#Duration">
        <rdfs:subClassOf rdf:resource="http://www.w3.org/2006/time#TemporalDuration"/>
        <rdfs:subClassOf>
            <owl:Restriction>
                <owl:onProperty rdf:resource="http://www.w3.org/2006/time#unitType"/>
                <owl:cardinality rdf:datatype="http://www.w3.org/2001/XMLSchema#nonNegativeInteger">1</owl:cardinality>
            </owl:Restriction>
        </rdfs:subClassOf>
        <rdfs:subClassOf>
            <owl:Restriction>
                <owl:onProperty rdf:resource="http://www.w3.org/2006/time#numericDuration"/>
                <owl:cardinality rdf:datatype="http://www.w3.org/2001/XMLSchema#nonNegativeInteger">1</owl:cardinality>
            </owl:Restriction>
        </rdfs:subClassOf>
        <rdfs:comment xml:lang="es">Duraci�n de una extensi�n temporal expresada como un n�mero escalado por una unidad temporal.</rdfs:comment>
        <rdfs:comment xml:lang="en">Duration of a temporal extent expressed as a number scaled by a temporal unit</rdfs:comment>
        <rdfs:label xml:lang="en">Time duration</rdfs:label>
        <rdfs:label>duraci�n de tiempo</rdfs:label>
        <skos:definition xml:lang="es">Duraci�n de una extensi�n temporal expresada como un n�mero escalado por una unidad temporal.</skos:definition>
        <skos:definition xml:lang="en">Duration of a temporal extent expressed as a number scaled by a temporal unit</skos:definition>
        <skos:note xml:lang="es">Alternativa a &apos;descripci�n de tiempo&apos; para proporcionar descripci�n soporte a una duraci�n temporal diferente a utilizar un sistema de calendario/reloj.</skos:note>
        <skos:note xml:lang="en">Alternative to time:DurationDescription to support description of a temporal duration other than using a calendar/clock system.</skos:note>
    </owl:Class>
    


    <!-- http://www.w3.org/2006/time#DurationDescription -->

    <owl:Class rdf:about="http://www.w3.org/2006/time#DurationDescription">
        <rdfs:subClassOf rdf:resource="http://www.w3.org/2006/time#GeneralDurationDescription"/>
        <rdfs:subClassOf>
            <owl:Restriction>
                <owl:onProperty rdf:resource="http://www.w3.org/2006/time#hasTRS"/>
                <owl:hasValue rdf:resource="http://www.opengis.net/def/uom/ISO-8601/0/Gregorian"/>
            </owl:Restriction>
        </rdfs:subClassOf>
        <rdfs:subClassOf>
            <owl:Restriction>
                <owl:onProperty rdf:resource="http://www.w3.org/2006/time#days"/>
                <owl:allValuesFrom rdf:resource="http://www.w3.org/2001/XMLSchema#decimal"/>
            </owl:Restriction>
        </rdfs:subClassOf>
        <rdfs:subClassOf>
            <owl:Restriction>
                <owl:onProperty rdf:resource="http://www.w3.org/2006/time#hours"/>
                <owl:allValuesFrom rdf:resource="http://www.w3.org/2001/XMLSchema#decimal"/>
            </owl:Restriction>
        </rdfs:subClassOf>
        <rdfs:subClassOf>
            <owl:Restriction>
                <owl:onProperty rdf:resource="http://www.w3.org/2006/time#minutes"/>
                <owl:allValuesFrom rdf:resource="http://www.w3.org/2001/XMLSchema#decimal"/>
            </owl:Restriction>
        </rdfs:subClassOf>
        <rdfs:subClassOf>
            <owl:Restriction>
                <owl:onProperty rdf:resource="http://www.w3.org/2006/time#months"/>
                <owl:allValuesFrom rdf:resource="http://www.w3.org/2001/XMLSchema#decimal"/>
            </owl:Restriction>
        </rdfs:subClassOf>
        <rdfs:subClassOf>
            <owl:Restriction>
                <owl:onProperty rdf:resource="http://www.w3.org/2006/time#seconds"/>
                <owl:allValuesFrom rdf:resource="http://www.w3.org/2001/XMLSchema#decimal"/>
            </owl:Restriction>
        </rdfs:subClassOf>
        <rdfs:subClassOf>
            <owl:Restriction>
                <owl:onProperty rdf:resource="http://www.w3.org/2006/time#weeks"/>
                <owl:allValuesFrom rdf:resource="http://www.w3.org/2001/XMLSchema#decimal"/>
            </owl:Restriction>
        </rdfs:subClassOf>
        <rdfs:subClassOf>
            <owl:Restriction>
                <owl:onProperty rdf:resource="http://www.w3.org/2006/time#years"/>
                <owl:allValuesFrom rdf:resource="http://www.w3.org/2001/XMLSchema#decimal"/>
            </owl:Restriction>
        </rdfs:subClassOf>
        <rdfs:comment xml:lang="es">Descripci�n de extensi�n temporal estructurada con valores separados para los distintos elementos de un sistema de horario-calendario. El sistema de referencia temporal se fija al calendario gregoriano, y el intervalo de cada una de las propiedades num�ricas se restringe a xsd:decimal.</rdfs:comment>
        <rdfs:comment xml:lang="en">Description of temporal extent structured with separate values for the various elements of a calendar-clock system. The temporal reference system is fixed to Gregorian Calendar, and the range of each of the numeric properties is restricted to xsd:decimal</rdfs:comment>
        <rdfs:label xml:lang="en">Duration description</rdfs:label>
        <rdfs:label xml:lang="es">descripci�n de duraci�n</rdfs:label>
        <skos:definition xml:lang="es">Descripci�n de extensi�n temporal estructurada con valores separados para los distintos elementos de un sistema de horario-calendario. El sistema de referencia temporal se fija al calendario gregoriano, y el intervalo de cada una de las propiedades num�ricas se restringe a xsd:decimal.</skos:definition>
        <skos:definition xml:lang="en">Description of temporal extent structured with separate values for the various elements of a calendar-clock system. The temporal reference system is fixed to Gregorian Calendar, and the range of each of the numeric properties is restricted to xsd:decimal</skos:definition>
        <skos:note xml:lang="es">En el calendario gregoriano la longitud de los meses no es fija. Por lo tanto, un valor como &quot;2,5 meses&quot; no se puede comparar exactamente con una duraci�n similar expresada en t�rminos de semanas o d�as.</skos:note>
        <skos:note xml:lang="en">In the Gregorian calendar the length of the month is not fixed. Therefore, a value like &quot;2.5 months&quot; cannot be exactly compared with a similar duration expressed in terms of weeks or days.</skos:note>
    </owl:Class>
    


    <!-- http://www.w3.org/2006/time#GeneralDateTimeDescription -->

    <owl:Class rdf:about="http://www.w3.org/2006/time#GeneralDateTimeDescription">
        <rdfs:subClassOf rdf:resource="http://www.w3.org/2006/time#TemporalPosition"/>
        <rdfs:subClassOf>
            <owl:Restriction>
                <owl:onProperty rdf:resource="http://www.w3.org/2006/time#unitType"/>
                <owl:cardinality rdf:datatype="http://www.w3.org/2001/XMLSchema#nonNegativeInteger">1</owl:cardinality>
            </owl:Restriction>
        </rdfs:subClassOf>
        <rdfs:subClassOf>
            <owl:Restriction>
                <owl:onProperty rdf:resource="http://www.w3.org/2006/time#dayOfWeek"/>
                <owl:maxCardinality rdf:datatype="http://www.w3.org/2001/XMLSchema#nonNegativeInteger">1</owl:maxCardinality>
            </owl:Restriction>
        </rdfs:subClassOf>
        <rdfs:subClassOf>
            <owl:Restriction>
                <owl:onProperty rdf:resource="http://www.w3.org/2006/time#monthOfYear"/>
                <owl:maxCardinality rdf:datatype="http://www.w3.org/2001/XMLSchema#nonNegativeInteger">1</owl:maxCardinality>
            </owl:Restriction>
        </rdfs:subClassOf>
        <rdfs:subClassOf>
            <owl:Restriction>
                <owl:onProperty rdf:resource="http://www.w3.org/2006/time#timeZone"/>
                <owl:maxCardinality rdf:datatype="http://www.w3.org/2001/XMLSchema#nonNegativeInteger">1</owl:maxCardinality>
            </owl:Restriction>
        </rdfs:subClassOf>
        <rdfs:subClassOf>
            <owl:Restriction>
                <owl:onProperty rdf:resource="http://www.w3.org/2006/time#day"/>
                <owl:maxCardinality rdf:datatype="http://www.w3.org/2001/XMLSchema#nonNegativeInteger">1</owl:maxCardinality>
            </owl:Restriction>
        </rdfs:subClassOf>
        <rdfs:subClassOf>
            <owl:Restriction>
                <owl:onProperty rdf:resource="http://www.w3.org/2006/time#dayOfYear"/>
                <owl:maxCardinality rdf:datatype="http://www.w3.org/2001/XMLSchema#nonNegativeInteger">1</owl:maxCardinality>
            </owl:Restriction>
        </rdfs:subClassOf>
        <rdfs:subClassOf>
            <owl:Restriction>
                <owl:onProperty rdf:resource="http://www.w3.org/2006/time#hour"/>
                <owl:maxCardinality rdf:datatype="http://www.w3.org/2001/XMLSchema#nonNegativeInteger">1</owl:maxCardinality>
            </owl:Restriction>
        </rdfs:subClassOf>
        <rdfs:subClassOf>
            <owl:Restriction>
                <owl:onProperty rdf:resource="http://www.w3.org/2006/time#minute"/>
                <owl:maxCardinality rdf:datatype="http://www.w3.org/2001/XMLSchema#nonNegativeInteger">1</owl:maxCardinality>
            </owl:Restriction>
        </rdfs:subClassOf>
        <rdfs:subClassOf>
            <owl:Restriction>
                <owl:onProperty rdf:resource="http://www.w3.org/2006/time#month"/>
                <owl:maxCardinality rdf:datatype="http://www.w3.org/2001/XMLSchema#nonNegativeInteger">1</owl:maxCardinality>
            </owl:Restriction>
        </rdfs:subClassOf>
        <rdfs:subClassOf>
            <owl:Restriction>
                <owl:onProperty rdf:resource="http://www.w3.org/2006/time#second"/>
                <owl:maxCardinality rdf:datatype="http://www.w3.org/2001/XMLSchema#nonNegativeInteger">1</owl:maxCardinality>
            </owl:Restriction>
        </rdfs:subClassOf>
        <rdfs:subClassOf>
            <owl:Restriction>
                <owl:onProperty rdf:resource="http://www.w3.org/2006/time#week"/>
                <owl:maxCardinality rdf:datatype="http://www.w3.org/2001/XMLSchema#nonNegativeInteger">1</owl:maxCardinality>
            </owl:Restriction>
        </rdfs:subClassOf>
        <rdfs:subClassOf>
            <owl:Restriction>
                <owl:onProperty rdf:resource="http://www.w3.org/2006/time#year"/>
                <owl:maxCardinality rdf:datatype="http://www.w3.org/2001/XMLSchema#nonNegativeInteger">1</owl:maxCardinality>
            </owl:Restriction>
        </rdfs:subClassOf>
        <rdfs:comment xml:lang="es">Descripci�n de fecha y hora estructurada con valores separados para los distintos elementos de un sistema calendario-reloj.</rdfs:comment>
        <rdfs:comment xml:lang="en">Description of date and time structured with separate values for the various elements of a calendar-clock system</rdfs:comment>
        <rdfs:label xml:lang="en">Generalized date-time description</rdfs:label>
        <rdfs:label xml:lang="es">descripci�n de fecha-hora generalizada</rdfs:label>
        <skos:definition>Descripci�n de fecha y hora estructurada con valores separados para los distintos elementos de un sistema calendario-reloj.</skos:definition>
        <skos:definition xml:lang="en">Description of date and time structured with separate values for the various elements of a calendar-clock system</skos:definition>
        <skos:note xml:lang="es">Algunas combinaciones de propiedades son redundantes - por ejemplo, dentro de un &apos;a�o&apos; especificado si se proporciona &apos;d�a del a�o&apos; entonces &apos;d�a&apos; y &apos;mes&apos; se pueden computar, y viceversa. Los valores individuales deber�an ser consistentes entre ellos y con el calendario, indicado a trav�s del valor de la propiedad &apos;tiene TRS&apos;.</skos:note>
        <skos:note>Some combinations of properties are redundant - for example, within a specified :year if :dayOfYear is provided then :day and :month can be computed, and vice versa. Individual values should be consistent with each other and the calendar, indicated through the value of the :hasTRS property.</skos:note>
    </owl:Class>
    


    <!-- http://www.w3.org/2006/time#GeneralDurationDescription -->

    <owl:Class rdf:about="http://www.w3.org/2006/time#GeneralDurationDescription">
        <rdfs:subClassOf rdf:resource="http://www.w3.org/2006/time#TemporalDuration"/>
        <rdfs:subClassOf>
            <owl:Restriction>
                <owl:onProperty rdf:resource="http://www.w3.org/2006/time#hasTRS"/>
                <owl:cardinality rdf:datatype="http://www.w3.org/2001/XMLSchema#nonNegativeInteger">1</owl:cardinality>
            </owl:Restriction>
        </rdfs:subClassOf>
        <rdfs:subClassOf>
            <owl:Restriction>
                <owl:onProperty rdf:resource="http://www.w3.org/2006/time#days"/>
                <owl:maxCardinality rdf:datatype="http://www.w3.org/2001/XMLSchema#nonNegativeInteger">1</owl:maxCardinality>
            </owl:Restriction>
        </rdfs:subClassOf>
        <rdfs:subClassOf>
            <owl:Restriction>
                <owl:onProperty rdf:resource="http://www.w3.org/2006/time#hours"/>
                <owl:maxCardinality rdf:datatype="http://www.w3.org/2001/XMLSchema#nonNegativeInteger">1</owl:maxCardinality>
            </owl:Restriction>
        </rdfs:subClassOf>
        <rdfs:subClassOf>
            <owl:Restriction>
                <owl:onProperty rdf:resource="http://www.w3.org/2006/time#minutes"/>
                <owl:maxCardinality rdf:datatype="http://www.w3.org/2001/XMLSchema#nonNegativeInteger">1</owl:maxCardinality>
            </owl:Restriction>
        </rdfs:subClassOf>
        <rdfs:subClassOf>
            <owl:Restriction>
                <owl:onProperty rdf:resource="http://www.w3.org/2006/time#months"/>
                <owl:maxCardinality rdf:datatype="http://www.w3.org/2001/XMLSchema#nonNegativeInteger">1</owl:maxCardinality>
            </owl:Restriction>
        </rdfs:subClassOf>
        <rdfs:subClassOf>
            <owl:Restriction>
                <owl:onProperty rdf:resource="http://www.w3.org/2006/time#seconds"/>
                <owl:maxCardinality rdf:datatype="http://www.w3.org/2001/XMLSchema#nonNegativeInteger">1</owl:maxCardinality>
            </owl:Restriction>
        </rdfs:subClassOf>
        <rdfs:subClassOf>
            <owl:Restriction>
                <owl:onProperty rdf:resource="http://www.w3.org/2006/time#weeks"/>
                <owl:maxCardinality rdf:datatype="http://www.w3.org/2001/XMLSchema#nonNegativeInteger">1</owl:maxCardinality>
            </owl:Restriction>
        </rdfs:subClassOf>
        <rdfs:subClassOf>
            <owl:Restriction>
                <owl:onProperty rdf:resource="http://www.w3.org/2006/time#years"/>
                <owl:maxCardinality rdf:datatype="http://www.w3.org/2001/XMLSchema#nonNegativeInteger">1</owl:maxCardinality>
            </owl:Restriction>
        </rdfs:subClassOf>
        <rdfs:comment xml:lang="es">Descripci�n de extensi�n temporal estructurada con valores separados para los distintos elementos de un sistema de horario-calendario.</rdfs:comment>
        <rdfs:comment xml:lang="en">Description of temporal extent structured with separate values for the various elements of a calendar-clock system.</rdfs:comment>
        <rdfs:label xml:lang="en">Generalized duration description</rdfs:label>
        <rdfs:label xml:lang="es">descripci�n de duraci�n generalizada</rdfs:label>
        <skos:definition xml:lang="es">Descripci�n de extensi�n temporal estructurada con valores separados para los distintos elementos de un sistema de horario-calendario.</skos:definition>
        <skos:definition xml:lang="en">Description of temporal extent structured with separate values for the various elements of a calendar-clock system.</skos:definition>
        <skos:note xml:lang="es">La extensi�n de una duraci�n de tiempo expresada como una &apos;descripci�n de duraci�n general&apos; depende del Sistema de Referencia Temporal. En algunos calendarios la longitud de la semana o del mes no es constante a lo largo del a�o. Por tanto, un valor como &quot;25 meses&quot; puede no ser necesariamente ser comparado con un duraci�n similar expresada en t�rminos de semanas o d�as. Cuando se consideran calendarios que no est�n basados en el movimiento de la Tierra, se deben tomar incluso m�s precauciones en la comparaci�n de duraciones.</skos:note>
        <skos:note xml:lang="en">The extent of a time duration expressed as a GeneralDurationDescription depends on the Temporal Reference System. In some calendars the length of the week or month is not constant within the year. Therefore, a value like &quot;2.5 months&quot; may not necessarily be exactly compared with a similar duration expressed in terms of weeks or days. When non-earth-based calendars are considered even more care must be taken in comparing durations.</skos:note>
    </owl:Class>
    


    <!-- http://www.w3.org/2006/time#Instant -->

    <owl:Class rdf:about="http://www.w3.org/2006/time#Instant">
        <rdfs:subClassOf rdf:resource="http://www.w3.org/2006/time#TemporalEntity"/>
        <owl:disjointWith rdf:resource="http://www.w3.org/2006/time#ProperInterval"/>
        <rdfs:comment xml:lang="en">A temporal entity with zero extent or duration</rdfs:comment>
        <rdfs:comment xml:lang="es">Una entidad temporal con una extensi�n o duraci�n cero.</rdfs:comment>
        <rdfs:label xml:lang="en">Time instant</rdfs:label>
        <rdfs:label xml:lang="es">instante de tiempo.</rdfs:label>
        <skos:definition xml:lang="en">A temporal entity with zero extent or duration</skos:definition>
        <skos:definition xml:lang="es">Una entidad temporal con una extensi�n o duraci�n cero.</skos:definition>
    </owl:Class>
    


    <!-- http://www.w3.org/2006/time#Interval -->

    <owl:Class rdf:about="http://www.w3.org/2006/time#Interval">
        <rdfs:subClassOf rdf:resource="http://www.w3.org/2006/time#TemporalEntity"/>
        <rdfs:comment xml:lang="en">A temporal entity with an extent or duration</rdfs:comment>
        <rdfs:comment xml:lang="es">Una entidad temporal con una extensi�n o duraci�n.</rdfs:comment>
        <rdfs:label xml:lang="en">Time interval</rdfs:label>
        <rdfs:label xml:lang="es">intervalo de tiempo</rdfs:label>
        <skos:definition xml:lang="en">A temporal entity with an extent or duration</skos:definition>
        <skos:definition xml:lang="es">Una entidad temporal con una extensi�n o duraci�n.</skos:definition>
    </owl:Class>
    


    <!-- http://www.w3.org/2006/time#January -->

    <owl:Class rdf:about="http://www.w3.org/2006/time#January">
        <rdfs:subClassOf rdf:resource="http://www.w3.org/2006/time#DateTimeDescription"/>
        <rdfs:subClassOf>
            <owl:Restriction>
                <owl:onProperty rdf:resource="http://www.w3.org/2006/time#unitType"/>
                <owl:hasValue rdf:resource="http://www.w3.org/2006/time#unitMonth"/>
            </owl:Restriction>
        </rdfs:subClassOf>
        <rdfs:subClassOf>
            <owl:Restriction>
                <owl:onProperty rdf:resource="http://www.w3.org/2006/time#month"/>
                <owl:hasValue>--01</owl:hasValue>
            </owl:Restriction>
        </rdfs:subClassOf>
        <rdfs:label>January</rdfs:label>
        <owl:deprecated rdf:datatype="http://www.w3.org/2001/XMLSchema#boolean">true</owl:deprecated>
        <skos:historyNote>This class was present in the 2006 version of OWL-Time. It was presented as an example of how DateTimeDescription could be specialized, but does not belong in the revised ontology. </skos:historyNote>
    </owl:Class>
    


    <!-- http://www.w3.org/2006/time#MonthOfYear -->

    <owl:Class rdf:about="http://www.w3.org/2006/time#MonthOfYear">
        <rdfs:subClassOf rdf:resource="http://www.w3.org/2006/time#DateTimeDescription"/>
        <rdfs:subClassOf>
            <owl:Restriction>
                <owl:onProperty rdf:resource="http://www.w3.org/2006/time#unitType"/>
                <owl:hasValue rdf:resource="http://www.w3.org/2006/time#unitMonth"/>
            </owl:Restriction>
        </rdfs:subClassOf>
        <rdfs:subClassOf>
            <owl:Restriction>
                <owl:onProperty rdf:resource="http://www.w3.org/2006/time#day"/>
                <owl:cardinality rdf:datatype="http://www.w3.org/2001/XMLSchema#nonNegativeInteger">0</owl:cardinality>
            </owl:Restriction>
        </rdfs:subClassOf>
        <rdfs:subClassOf>
            <owl:Restriction>
                <owl:onProperty rdf:resource="http://www.w3.org/2006/time#hour"/>
                <owl:cardinality rdf:datatype="http://www.w3.org/2001/XMLSchema#nonNegativeInteger">0</owl:cardinality>
            </owl:Restriction>
        </rdfs:subClassOf>
        <rdfs:subClassOf>
            <owl:Restriction>
                <owl:onProperty rdf:resource="http://www.w3.org/2006/time#minute"/>
                <owl:cardinality rdf:datatype="http://www.w3.org/2001/XMLSchema#nonNegativeInteger">0</owl:cardinality>
            </owl:Restriction>
        </rdfs:subClassOf>
        <rdfs:subClassOf>
            <owl:Restriction>
                <owl:onProperty rdf:resource="http://www.w3.org/2006/time#month"/>
                <owl:cardinality rdf:datatype="http://www.w3.org/2001/XMLSchema#nonNegativeInteger">1</owl:cardinality>
            </owl:Restriction>
        </rdfs:subClassOf>
        <rdfs:subClassOf>
            <owl:Restriction>
                <owl:onProperty rdf:resource="http://www.w3.org/2006/time#second"/>
                <owl:cardinality rdf:datatype="http://www.w3.org/2001/XMLSchema#nonNegativeInteger">0</owl:cardinality>
            </owl:Restriction>
        </rdfs:subClassOf>
        <rdfs:subClassOf>
            <owl:Restriction>
                <owl:onProperty rdf:resource="http://www.w3.org/2006/time#week"/>
                <owl:cardinality rdf:datatype="http://www.w3.org/2001/XMLSchema#nonNegativeInteger">0</owl:cardinality>
            </owl:Restriction>
        </rdfs:subClassOf>
        <rdfs:subClassOf>
            <owl:Restriction>
                <owl:onProperty rdf:resource="http://www.w3.org/2006/time#year"/>
                <owl:cardinality rdf:datatype="http://www.w3.org/2001/XMLSchema#nonNegativeInteger">0</owl:cardinality>
            </owl:Restriction>
        </rdfs:subClassOf>
        <rdfs:comment xml:lang="es">El mes del a�o.</rdfs:comment>
        <rdfs:comment xml:lang="en">The month of the year</rdfs:comment>
        <rdfs:label xml:lang="en">Month of year</rdfs:label>
        <rdfs:label xml:lang="es">mes del a�o</rdfs:label>
        <skos:definition xml:lang="es">El mes del a�o.</skos:definition>
        <skos:definition xml:lang="en">The month of the year</skos:definition>
        <skos:editorialNote xml:lang="es">Caracter�stica en riesgo - a�adida en la revisi�n de 2017, y no utilizada todav�a de forma amplia.</skos:editorialNote>
        <skos:editorialNote xml:lang="en">Feature at risk - added in 2017 revision, and not yet widely used. </skos:editorialNote>
        <skos:note xml:lang="es">La pertenencia a la clase &apos;mes del a�o&apos; est� abierta, a permitir calendarios anuales alternativos y diferentes nombres de meses.</skos:note>
        <skos:note xml:lang="en">Membership of the class :MonthOfYear is open, to allow for alternative annual calendars and different month names.</skos:note>
    </owl:Class>
    


    <!-- http://www.w3.org/2006/time#ProperInterval -->

    <owl:Class rdf:about="http://www.w3.org/2006/time#ProperInterval">
        <rdfs:subClassOf rdf:resource="http://www.w3.org/2006/time#Interval"/>
        <rdfs:comment xml:lang="en">A temporal entity with non-zero extent or duration, i.e. for which the value of the beginning and end are different</rdfs:comment>
        <rdfs:comment xml:lang="es">Una entidad temporal con extensi�n o duraci�n distinta de cero, es decir, para la cual los valores de principio y fin del intervalo son diferentes.</rdfs:comment>
        <rdfs:label xml:lang="en">Proper interval</rdfs:label>
        <rdfs:label xml:lang="es">intervalo propio</rdfs:label>
        <skos:definition xml:lang="en">A temporal entity with non-zero extent or duration, i.e. for which the value of the beginning and end are different</skos:definition>
        <skos:definition xml:lang="es">Una entidad temporal con extensi�n o duraci�n distinta de cero, es decir, para la cual los valores de principio y fin del intervalo son diferentes.</skos:definition>
    </owl:Class>
    


    <!-- http://www.w3.org/2006/time#TRS -->

    <owl:Class rdf:about="http://www.w3.org/2006/time#TRS">
        <rdfs:comment xml:lang="en">A temporal reference system, such as a temporal coordinate system (with an origin, direction, and scale), a calendar-clock combination, or a (possibly hierarchical) ordinal system. 

This is a stub class, representing the set of all temporal reference systems.</rdfs:comment>
        <rdfs:comment xml:lang="es">Un sistema de referencia temporal, tal como un sistema de coordenadas temporales (con un origen, una direcci�n y una escala), una combinaci�n calendario-reloj, o un sistema ordinal (posiblemente jer�rquico).
        Esta clase comod�n representa el conjunto de todos los sistemas de referencia temporal.</rdfs:comment>
        <rdfs:label xml:lang="en">Temporal Reference System</rdfs:label>
        <rdfs:label xml:lang="es">sistema de referencia temporal</rdfs:label>
        <skos:definition xml:lang="en">A temporal reference system, such as a temporal coordinate system (with an origin, direction, and scale), a calendar-clock combination, or a (possibly hierarchical) ordinal system. 

This is a stub class, representing the set of all temporal reference systems.</skos:definition>
        <skos:definition xml:lang="es">Un sistema de referencia temporal, tal como un sistema de coordenadas temporales (con un origen, una direcci�n y una escala), una combinaci�n calendario-reloj, o un sistema ordinal (posiblemente jer�rquico).
    Esta clase comod�n representa el conjunto de todos los sistemas de referencia temporal.</skos:definition>
        <skos:note xml:lang="en">A taxonomy of temporal reference systems is provided in ISO 19108:2002 [ISO19108], including (a) calendar + clock systems; (b) temporal coordinate systems (i.e. numeric offset from an epoch); (c) temporal ordinal reference systems (i.e. ordered sequence of named intervals, not necessarily of equal duration).</skos:note>
        <skos:note xml:lang="es">En el ISO 19108:2002 [ISO19108] se proporciona una taxonom�a de sistemas de referencia temporal, incluyendo (a) sistemas de calendario + reloj; (b) sistemas de coordenadas temporales (es decir, desplazamiento num�rico a partir de una �poca); (c) sistemas de referencia ordinales temporales (es decir, secuencia ordenada de intervalos nombrados, no necesariamente de igual duraci�n).</skos:note>
    </owl:Class>
    


    <!-- http://www.w3.org/2006/time#TemporalDuration -->

    <owl:Class rdf:about="http://www.w3.org/2006/time#TemporalDuration">
        <rdfs:comment xml:lang="es">Extensi�n de tiempo; duraci�n de un intervalo de tiempo independiente de su posici�n de inicio particular.</rdfs:comment>
        <rdfs:comment xml:lang="en">Time extent; duration of a time interval separate from its particular start position</rdfs:comment>
        <rdfs:label xml:lang="en">Temporal duration</rdfs:label>
        <rdfs:label xml:lang="es">duraci�n temporal</rdfs:label>
        <skos:definition xml:lang="es">Extensi�n de tiempo; duraci�n de un intervalo de tiempo independiente de su posici�n de inicio particular.</skos:definition>
        <skos:definition xml:lang="en">Time extent; duration of a time interval separate from its particular start position</skos:definition>
    </owl:Class>
    


    <!-- http://www.w3.org/2006/time#TemporalEntity -->

    <owl:Class rdf:about="http://www.w3.org/2006/time#TemporalEntity">
        <owl:equivalentClass>
            <owl:Class>
                <owl:unionOf rdf:parseType="Collection">
                    <rdf:Description rdf:about="http://www.w3.org/2006/time#Instant"/>
                    <rdf:Description rdf:about="http://www.w3.org/2006/time#Interval"/>
                </owl:unionOf>
            </owl:Class>
        </owl:equivalentClass>
        <rdfs:subClassOf rdf:resource="http://www.w3.org/2002/07/owl#Thing"/>
        <rdfs:comment xml:lang="en">A temporal interval or instant.</rdfs:comment>
        <rdfs:comment xml:lang="es">Un intervalo temporal o un instante.</rdfs:comment>
        <rdfs:label xml:lang="en">Temporal entity</rdfs:label>
        <rdfs:label xml:lang="es">entidad temporal</rdfs:label>
        <skos:definition xml:lang="en">A temporal interval or instant.</skos:definition>
        <skos:definition xml:lang="es">Un intervalo temporal o un instante.</skos:definition>
    </owl:Class>
    


    <!-- http://www.w3.org/2006/time#TemporalPosition -->

    <owl:Class rdf:about="http://www.w3.org/2006/time#TemporalPosition">
        <rdfs:subClassOf>
            <owl:Restriction>
                <owl:onProperty rdf:resource="http://www.w3.org/2006/time#hasTRS"/>
                <owl:cardinality rdf:datatype="http://www.w3.org/2001/XMLSchema#nonNegativeInteger">1</owl:cardinality>
            </owl:Restriction>
        </rdfs:subClassOf>
        <rdfs:comment xml:lang="en">A position on a time-line</rdfs:comment>
        <rdfs:comment xml:lang="es">Una posici�n sobre una l�nea de tiempo.</rdfs:comment>
        <rdfs:label xml:lang="en">Temporal position</rdfs:label>
        <rdfs:label xml:lang="es">posici�n temporal</rdfs:label>
        <skos:definition xml:lang="en">A position on a time-line</skos:definition>
        <skos:definition xml:lang="es">Una posici�n sobre una l�nea de tiempo.</skos:definition>
    </owl:Class>
    


    <!-- http://www.w3.org/2006/time#TemporalUnit -->

    <owl:Class rdf:about="http://www.w3.org/2006/time#TemporalUnit">
        <rdfs:subClassOf rdf:resource="http://www.w3.org/2006/time#TemporalDuration"/>
        <rdfs:comment xml:lang="en">A standard duration, which provides a scale factor for a time extent, or the granularity or precision for a time position.</rdfs:comment>
        <rdfs:comment xml:lang="es">Una duraci�n est�ndar, que proporciona un factor de escala para una extensi�n de tiempo, o la granularidad o precisi�n para una posici�n de tiempo.</rdfs:comment>
        <rdfs:label xml:lang="en">Temporal unit</rdfs:label>
        <rdfs:label xml:lang="es">unidad de tiempo</rdfs:label>
        <skos:changeNote xml:lang="en">Remove enumeration from definition, in order to allow other units to be used when required in other coordinate systems. 
NOTE: existing units are still present as members of the class, but the class membership is now open. 

In the original OWL-Time the following constraint appeared: 
  owl:oneOf (
      time:unitSecond
      time:unitMinute
      time:unitHour
      time:unitDay
      time:unitWeek
      time:unitMonth
      time:unitYear
    ) ;</skos:changeNote>
        <skos:definition xml:lang="en">A standard duration, which provides a scale factor for a time extent, or the granularity or precision for a time position.</skos:definition>
        <skos:definition xml:lang="es">Una duraci�n est�ndar, que proporciona un factor de escala para una extensi�n de tiempo, o la granularidad o precisi�n para una posici�n de tiempo.</skos:definition>
        <skos:note xml:lang="es">La pertenencia de la clase &apos;unidad de tiempo&apos; est� abierta, para permitir otras unidades de tiempo utilizadas en algunas aplicaciones t�cnicas (por ejemplo, millones de a�os o el mes Baha&apos;i).</skos:note>
        <skos:note xml:lang="en">Membership of the class TemporalUnit is open, to allow for other temporal units used in some technical applications (e.g. millions of years, Baha&apos;i month).</skos:note>
    </owl:Class>
    


    <!-- http://www.w3.org/2006/time#TimePosition -->

    <owl:Class rdf:about="http://www.w3.org/2006/time#TimePosition">
        <rdfs:subClassOf rdf:resource="http://www.w3.org/2006/time#TemporalPosition"/>
        <rdfs:subClassOf>
            <owl:Class>
                <owl:unionOf rdf:parseType="Collection">
                    <owl:Restriction>
                        <owl:onProperty rdf:resource="http://www.w3.org/2006/time#nominalPosition"/>
                        <owl:cardinality rdf:datatype="http://www.w3.org/2001/XMLSchema#nonNegativeInteger">1</owl:cardinality>
                    </owl:Restriction>
                    <owl:Restriction>
                        <owl:onProperty rdf:resource="http://www.w3.org/2006/time#numericPosition"/>
                        <owl:cardinality rdf:datatype="http://www.w3.org/2001/XMLSchema#nonNegativeInteger">1</owl:cardinality>
                    </owl:Restriction>
                </owl:unionOf>
            </owl:Class>
        </rdfs:subClassOf>
        <rdfs:comment xml:lang="en">A temporal position described using either a (nominal) value from an ordinal reference system, or a (numeric) value in a temporal coordinate system. </rdfs:comment>
        <rdfs:comment xml:lang="es">Una posici�n temporal descrita utilizando bien un valor (nominal) de un sistema de referencia ordinal, o un valor (num�rico) en un sistema de coordenadas temporales.</rdfs:comment>
        <rdfs:label xml:lang="en">Time position</rdfs:label>
        <rdfs:label xml:lang="es">posici�n de tiempo</rdfs:label>
        <skos:definition xml:lang="en">A temporal position described using either a (nominal) value from an ordinal reference system, or a (numeric) value in a temporal coordinate system. </skos:definition>
        <skos:definition xml:lang="es">Una posici�n temporal descrita utilizando bien un valor (nominal) de un sistema de referencia ordinal, o un valor (num�rico) en un sistema de coordenadas temporales.</skos:definition>
    </owl:Class>
    


    <!-- http://www.w3.org/2006/time#TimeZone -->

    <owl:Class rdf:about="http://www.w3.org/2006/time#TimeZone">
        <rdfs:comment xml:lang="en">A Time Zone specifies the amount by which the local time is offset from UTC. 
	A time zone is usually denoted geographically (e.g. Australian Eastern Daylight Time), with a constant value in a given region. 
The region where it applies and the offset from UTC are specified by a locally recognised governing authority.</rdfs:comment>
        <rdfs:comment xml:lang="es">Un huso horario especifica la cantidad en que la hora local est� desplazada con respecto a UTC.
        Un huso horario normalmente se denota geogr�ficamente (p.ej. el horario de verano del este de Australia), con un valor constante en una regi�n dada.
        La regi�n donde aplica y el desplazamiento desde UTC las especifica una autoridad gubernamental localmente reconocida.</rdfs:comment>
        <rdfs:label xml:lang="en">Time Zone</rdfs:label>
        <rdfs:label xml:lang="es">huso horario</rdfs:label>
        <skos:definition xml:lang="en">A Time Zone specifies the amount by which the local time is offset from UTC. 
	A time zone is usually denoted geographically (e.g. Australian Eastern Daylight Time), with a constant value in a given region. 
The region where it applies and the offset from UTC are specified by a locally recognised governing authority.</skos:definition>
        <skos:definition xml:lang="es">Un huso horario especifica la cantidad en que la hora local est� desplazada con respecto a UTC.
    Un huso horario normalmente se denota geogr�ficamente (p.ej. el horario de verano del este de Australia), con un valor constante en una regi�n dada.
    La regi�n donde aplica y el desplazamiento desde UTC las especifica una autoridad gubernamental localmente reconocida.</skos:definition>
        <skos:historyNote xml:lang="es">En la versi�n original de OWL-Time de 2006, se defini�, en un espacio de nombres diferente &quot;http://www.w3.org/2006/timezone#&quot;, la clase &apos;huso horario&apos;, con varias propiedades espec�ficas correspondientes a un modelo espec�fico de huso horario.
    En la versi�n actual hay una clase con el mismo nombre local en el espacio de nombres de OWL-Time, eliminando la dependencia del espacio de nombres externo.
    Un axioma de alineaci�n permite que los datos codificados de acuerdo con la versi�n anterior sean consistentes con la ontolog�a actualizada.</skos:historyNote>
        <skos:historyNote>In the original 2006 version of OWL-Time, the TimeZone class, with several properties corresponding to a specific model of time-zones, was defined in a separate namespace &quot;http://www.w3.org/2006/timezone#&quot;. 

In the current version a class with same local name is put into the main OWL-Time namespace, removing the dependency on the external namespace. 

An alignment axiom 
	tzont:TimeZone rdfs:subClassOf time:TimeZone . 
allows data encoded according to the previous version to be consistent with the updated ontology. </skos:historyNote>
        <skos:note xml:lang="en">A designated timezone is associated with a geographic region. However, for a particular region the offset from UTC often varies seasonally, and the dates of the changes may vary from year to year. The timezone designation usually changes for the different seasons (e.g. Australian Eastern Standard Time vs. Australian Eastern Daylight Time). Furthermore, the offset for a timezone may change over longer timescales, though its designation might not.  

Detailed guidance about working with time zones is given in http://www.w3.org/TR/timezone/ .</skos:note>
        <skos:note xml:lang="en">An ontology for time zone descriptions was described in [owl-time-20060927] and provided as RDF in a separate namespace tzont:. However, that ontology was incomplete in scope, and the example datasets were selective. Furthermore, since the use of a class from an external ontology as the range of an ObjectProperty in OWL-Time creates a dependency, reference to the time zone class has been replaced with the &apos;stub&apos; class in the normative part of this version of OWL-Time.</skos:note>
        <skos:note xml:lang="es">Un huso horario designado est� asociado con una regi�n geogr�fica. Sin embargo, para una regi�n particular el desplazamiento desde UTC a menudo var�a seg�n las estaciones, y las fechas de los cambios pueden variar de un a�o a otro. La designaci�n de huso horario  normalmente cambia de una estaci�n a otra (por ejemplo, el horario est�ndar frente al horario de verano ambos del este de Australia). Adem�s, del desplazamiento para un huso horario puede cambiar sobre escalas de tiempo mayores, aunque su designaci�n no lo haga.
    Se puede encontrar una gu�a detallada sobre el funcionamiento de husos horarios en http://www.w3.org/TR/timezone/.&quot;@es , &quot;En [owl-time-20060927] se describi� una ontolog�a para descripciones de husos horarios, y se proporcion� en un espacio de nombres separado tzont:. Sin embargo, dicha ontolog�a estaba incompleta en su alcance, y el ejemplo de conjuntos de datos (datasets) era selectivo. Adem�s, puesto que el uso de una clase de una ontolog�a externa como el rango de una propiedad de objeto en OWL-Time crea una dependencia, la referencia a la clase huso horario se ha reemplazado por una clase que viene a ser un &quot;caj�n de sastre&quot; en la en la parte normativa de esta versi�n de OWL-Time.</skos:note>
        <skos:scopeNote xml:lang="es">En esta implementaci�n &apos;huso horario&apos; no tiene definidas propiedades. Se deber�a pensar como una superclase &quot;abstracta&quot; de todas las implementaciones de huso horario espec�ficas.</skos:scopeNote>
        <skos:scopeNote>In this implementation TimeZone has no properties defined. It should be thought of as an &apos;abstract&apos; superclass of all specific timezone implementations.</skos:scopeNote>
    </owl:Class>
    


    <!-- http://www.w3.org/2006/time#Year -->

    <owl:Class rdf:about="http://www.w3.org/2006/time#Year">
        <rdfs:subClassOf rdf:resource="http://www.w3.org/2006/time#DurationDescription"/>
        <rdfs:subClassOf>
            <owl:Restriction>
                <owl:onProperty rdf:resource="http://www.w3.org/2006/time#days"/>
                <owl:cardinality rdf:datatype="http://www.w3.org/2001/XMLSchema#nonNegativeInteger">0</owl:cardinality>
            </owl:Restriction>
        </rdfs:subClassOf>
        <rdfs:subClassOf>
            <owl:Restriction>
                <owl:onProperty rdf:resource="http://www.w3.org/2006/time#hours"/>
                <owl:cardinality rdf:datatype="http://www.w3.org/2001/XMLSchema#nonNegativeInteger">0</owl:cardinality>
            </owl:Restriction>
        </rdfs:subClassOf>
        <rdfs:subClassOf>
            <owl:Restriction>
                <owl:onProperty rdf:resource="http://www.w3.org/2006/time#minutes"/>
                <owl:cardinality rdf:datatype="http://www.w3.org/2001/XMLSchema#nonNegativeInteger">0</owl:cardinality>
            </owl:Restriction>
        </rdfs:subClassOf>
        <rdfs:subClassOf>
            <owl:Restriction>
                <owl:onProperty rdf:resource="http://www.w3.org/2006/time#months"/>
                <owl:cardinality rdf:datatype="http://www.w3.org/2001/XMLSchema#nonNegativeInteger">0</owl:cardinality>
            </owl:Restriction>
        </rdfs:subClassOf>
        <rdfs:subClassOf>
            <owl:Restriction>
                <owl:onProperty rdf:resource="http://www.w3.org/2006/time#seconds"/>
                <owl:cardinality rdf:datatype="http://www.w3.org/2001/XMLSchema#nonNegativeInteger">0</owl:cardinality>
            </owl:Restriction>
        </rdfs:subClassOf>
        <rdfs:subClassOf>
            <owl:Restriction>
                <owl:onProperty rdf:resource="http://www.w3.org/2006/time#weeks"/>
                <owl:cardinality rdf:datatype="http://www.w3.org/2001/XMLSchema#nonNegativeInteger">0</owl:cardinality>
            </owl:Restriction>
        </rdfs:subClassOf>
        <rdfs:subClassOf>
            <owl:Restriction>
                <owl:onProperty rdf:resource="http://www.w3.org/2006/time#years"/>
                <owl:cardinality rdf:datatype="http://www.w3.org/2001/XMLSchema#nonNegativeInteger">1</owl:cardinality>
            </owl:Restriction>
        </rdfs:subClassOf>
        <rdfs:comment>Year duration</rdfs:comment>
        <rdfs:label xml:lang="en">Year</rdfs:label>
        <owl:deprecated rdf:datatype="http://www.w3.org/2001/XMLSchema#boolean">true</owl:deprecated>
        <skos:definition>Year duration</skos:definition>
        <skos:historyNote>Year was proposed in the 2006 version of OWL-Time as an example of how DurationDescription could be specialized to allow for a duration to be restricted to a number of years. 

It is deprecated in this edition of OWL-Time. </skos:historyNote>
        <skos:prefLabel xml:lang="ja">?</skos:prefLabel>
        <skos:prefLabel xml:lang="zh">?</skos:prefLabel>
        <skos:prefLabel xml:lang="ar">???</skos:prefLabel>
        <skos:prefLabel xml:lang="ru">???</skos:prefLabel>
        <skos:prefLabel xml:lang="it">Anno</skos:prefLabel>
        <skos:prefLabel xml:lang="fr">Ann�e (calendrier)</skos:prefLabel>
        <skos:prefLabel xml:lang="pt">Ano</skos:prefLabel>
        <skos:prefLabel xml:lang="es">A�o</skos:prefLabel>
        <skos:prefLabel xml:lang="nl">Jaar</skos:prefLabel>
        <skos:prefLabel xml:lang="de">Jahr</skos:prefLabel>
        <skos:prefLabel xml:lang="pl">Rok</skos:prefLabel>
        <skos:prefLabel xml:lang="en">Year</skos:prefLabel>
    </owl:Class>
    


    <!-- 
    ///////////////////////////////////////////////////////////////////////////////////////
    //
    // Individuals
    //
    ///////////////////////////////////////////////////////////////////////////////////////
     -->

    


    <!-- http://www.opengis.net/def/uom/ISO-8601/0/Gregorian -->

    <owl:NamedIndividual rdf:about="http://www.opengis.net/def/uom/ISO-8601/0/Gregorian"/>
    


    <!-- http://www.w3.org/2006/time#Friday -->

    <owl:NamedIndividual rdf:about="http://www.w3.org/2006/time#Friday">
        <rdf:type rdf:resource="http://www.w3.org/2006/time#DayOfWeek"/>
        <rdfs:label xml:lang="en">Friday</rdfs:label>
        <skos:prefLabel xml:lang="ja">???</skos:prefLabel>
        <skos:prefLabel xml:lang="zh">???</skos:prefLabel>
        <skos:prefLabel xml:lang="ar">??????</skos:prefLabel>
        <skos:prefLabel xml:lang="ru">???????</skos:prefLabel>
        <skos:prefLabel xml:lang="de">Freitag</skos:prefLabel>
        <skos:prefLabel xml:lang="en">Friday</skos:prefLabel>
        <skos:prefLabel xml:lang="pl">Piatek</skos:prefLabel>
        <skos:prefLabel xml:lang="pt">Sexta-feira</skos:prefLabel>
        <skos:prefLabel xml:lang="fr">Vendredi</skos:prefLabel>
        <skos:prefLabel xml:lang="it">Venerd�</skos:prefLabel>
        <skos:prefLabel xml:lang="es">Viernes</skos:prefLabel>
        <skos:prefLabel xml:lang="nl">Vrijdag</skos:prefLabel>
    </owl:NamedIndividual>
    


    <!-- http://www.w3.org/2006/time#Monday -->

    <owl:NamedIndividual rdf:about="http://www.w3.org/2006/time#Monday">
        <rdf:type rdf:resource="http://www.w3.org/2006/time#DayOfWeek"/>
        <rdfs:label xml:lang="en">Monday</rdfs:label>
        <skos:prefLabel xml:lang="ja">???</skos:prefLabel>
        <skos:prefLabel xml:lang="zh">???</skos:prefLabel>
        <skos:prefLabel xml:lang="ar">???????</skos:prefLabel>
        <skos:prefLabel xml:lang="ru">???????????</skos:prefLabel>
        <skos:prefLabel xml:lang="fr">Lundi</skos:prefLabel>
        <skos:prefLabel xml:lang="it">Luned�</skos:prefLabel>
        <skos:prefLabel xml:lang="es">Lunes</skos:prefLabel>
        <skos:prefLabel xml:lang="nl">Maandag</skos:prefLabel>
        <skos:prefLabel xml:lang="en">Monday</skos:prefLabel>
        <skos:prefLabel xml:lang="de">Montag</skos:prefLabel>
        <skos:prefLabel xml:lang="pl">Poniedzialek</skos:prefLabel>
        <skos:prefLabel xml:lang="pt">Segunda-feira</skos:prefLabel>
    </owl:NamedIndividual>
    


    <!-- http://www.w3.org/2006/time#Saturday -->

    <owl:NamedIndividual rdf:about="http://www.w3.org/2006/time#Saturday">
        <rdf:type rdf:resource="http://www.w3.org/2006/time#DayOfWeek"/>
        <rdfs:label xml:lang="en">Saturday</rdfs:label>
        <skos:prefLabel xml:lang="ja">???</skos:prefLabel>
        <skos:prefLabel xml:lang="zh">???</skos:prefLabel>
        <skos:prefLabel xml:lang="ar">?????</skos:prefLabel>
        <skos:prefLabel xml:lang="ru">???????</skos:prefLabel>
        <skos:prefLabel xml:lang="it">Sabato</skos:prefLabel>
        <skos:prefLabel xml:lang="fr">Samedi</skos:prefLabel>
        <skos:prefLabel xml:lang="de">Samstag</skos:prefLabel>
        <skos:prefLabel xml:lang="en">Saturday</skos:prefLabel>
        <skos:prefLabel xml:lang="pl">Sobota</skos:prefLabel>
        <skos:prefLabel xml:lang="es">S�bado</skos:prefLabel>
        <skos:prefLabel xml:lang="pt">S�bado</skos:prefLabel>
        <skos:prefLabel xml:lang="nl">Zaterdag</skos:prefLabel>
    </owl:NamedIndividual>
    


    <!-- http://www.w3.org/2006/time#Sunday -->

    <owl:NamedIndividual rdf:about="http://www.w3.org/2006/time#Sunday">
        <rdf:type rdf:resource="http://www.w3.org/2006/time#DayOfWeek"/>
        <rdfs:label xml:lang="en">Sunday</rdfs:label>
        <skos:prefLabel xml:lang="ja">???</skos:prefLabel>
        <skos:prefLabel xml:lang="zh">???</skos:prefLabel>
        <skos:prefLabel xml:lang="ar">????? (???)</skos:prefLabel>
        <skos:prefLabel xml:lang="ru">???????????</skos:prefLabel>
        <skos:prefLabel xml:lang="fr">Dimanche</skos:prefLabel>
        <skos:prefLabel xml:lang="it">Domenica</skos:prefLabel>
        <skos:prefLabel xml:lang="es">Domingo</skos:prefLabel>
        <skos:prefLabel xml:lang="pt">Domingo</skos:prefLabel>
        <skos:prefLabel xml:lang="pl">Niedziela</skos:prefLabel>
        <skos:prefLabel xml:lang="de">Sonntag</skos:prefLabel>
        <skos:prefLabel xml:lang="en">Sunday</skos:prefLabel>
        <skos:prefLabel xml:lang="nl">Zondag</skos:prefLabel>
    </owl:NamedIndividual>
    


    <!-- http://www.w3.org/2006/time#Thursday -->

    <owl:NamedIndividual rdf:about="http://www.w3.org/2006/time#Thursday">
        <rdf:type rdf:resource="http://www.w3.org/2006/time#DayOfWeek"/>
        <rdfs:label xml:lang="en">Thursday</rdfs:label>
        <skos:prefLabel xml:lang="ja">???</skos:prefLabel>
        <skos:prefLabel xml:lang="zh">???</skos:prefLabel>
        <skos:prefLabel xml:lang="ar">??????</skos:prefLabel>
        <skos:prefLabel xml:lang="ru">???????</skos:prefLabel>
        <skos:prefLabel xml:lang="pl">Czwartek</skos:prefLabel>
        <skos:prefLabel xml:lang="nl">Donderdag</skos:prefLabel>
        <skos:prefLabel xml:lang="de">Donnerstag</skos:prefLabel>
        <skos:prefLabel xml:lang="it">Gioved�</skos:prefLabel>
        <skos:prefLabel xml:lang="fr">Jeudi</skos:prefLabel>
        <skos:prefLabel xml:lang="es">Jueves</skos:prefLabel>
        <skos:prefLabel xml:lang="pt">Quinta-feira</skos:prefLabel>
        <skos:prefLabel xml:lang="en">Thursday</skos:prefLabel>
    </owl:NamedIndividual>
    


    <!-- http://www.w3.org/2006/time#Tuesday -->

    <owl:NamedIndividual rdf:about="http://www.w3.org/2006/time#Tuesday">
        <rdf:type rdf:resource="http://www.w3.org/2006/time#DayOfWeek"/>
        <rdfs:label xml:lang="en">Tuesday</rdfs:label>
        <skos:prefLabel xml:lang="ja">???</skos:prefLabel>
        <skos:prefLabel xml:lang="zh">???</skos:prefLabel>
        <skos:prefLabel xml:lang="ru">???????</skos:prefLabel>
        <skos:prefLabel xml:lang="ar">????????</skos:prefLabel>
        <skos:prefLabel xml:lang="de">Dienstag</skos:prefLabel>
        <skos:prefLabel xml:lang="nl">Dinsdag</skos:prefLabel>
        <skos:prefLabel xml:lang="fr">Mardi</skos:prefLabel>
        <skos:prefLabel xml:lang="it">Marted�</skos:prefLabel>
        <skos:prefLabel xml:lang="es">Martes</skos:prefLabel>
        <skos:prefLabel xml:lang="pt">Ter�a-feira</skos:prefLabel>
        <skos:prefLabel xml:lang="en">Tuesday</skos:prefLabel>
        <skos:prefLabel xml:lang="pl">Wtorek</skos:prefLabel>
    </owl:NamedIndividual>
    


    <!-- http://www.w3.org/2006/time#Wednesday -->

    <owl:NamedIndividual rdf:about="http://www.w3.org/2006/time#Wednesday">
        <rdf:type rdf:resource="http://www.w3.org/2006/time#DayOfWeek"/>
        <rdfs:label xml:lang="en">Wednesday</rdfs:label>
        <skos:prefLabel xml:lang="ja">???</skos:prefLabel>
        <skos:prefLabel xml:lang="zh">???</skos:prefLabel>
        <skos:prefLabel xml:lang="ru">?????</skos:prefLabel>
        <skos:prefLabel xml:lang="ar">????????</skos:prefLabel>
        <skos:prefLabel xml:lang="it">Mercoled�</skos:prefLabel>
        <skos:prefLabel xml:lang="fr">Mercredi</skos:prefLabel>
        <skos:prefLabel xml:lang="de">Mittwoch</skos:prefLabel>
        <skos:prefLabel xml:lang="es">Mi�rcoles</skos:prefLabel>
        <skos:prefLabel xml:lang="pt">Quarta-feira</skos:prefLabel>
        <skos:prefLabel xml:lang="pl">Sroda</skos:prefLabel>
        <skos:prefLabel xml:lang="en">Wednesday</skos:prefLabel>
        <skos:prefLabel xml:lang="nl">Woensdag</skos:prefLabel>
    </owl:NamedIndividual>
    


    <!-- http://www.w3.org/2006/time#unitDay -->

    <owl:NamedIndividual rdf:about="http://www.w3.org/2006/time#unitDay">
        <rdf:type rdf:resource="http://www.w3.org/2006/time#TemporalUnit"/>
        <days rdf:datatype="http://www.w3.org/2001/XMLSchema#decimal">1</days>
        <hours rdf:datatype="http://www.w3.org/2001/XMLSchema#decimal">0</hours>
        <minutes rdf:datatype="http://www.w3.org/2001/XMLSchema#decimal">0</minutes>
        <months rdf:datatype="http://www.w3.org/2001/XMLSchema#decimal">0</months>
        <seconds rdf:datatype="http://www.w3.org/2001/XMLSchema#decimal">0</seconds>
        <weeks rdf:datatype="http://www.w3.org/2001/XMLSchema#decimal">0</weeks>
        <years rdf:datatype="http://www.w3.org/2001/XMLSchema#decimal">0</years>
        <rdfs:label xml:lang="en">Day (unit of temporal duration)</rdfs:label>
        <skos:prefLabel xml:lang="zh">??</skos:prefLabel>
        <skos:prefLabel xml:lang="ja">???</skos:prefLabel>
        <skos:prefLabel xml:lang="kr">???</skos:prefLabel>
        <skos:prefLabel xml:lang="ar">????? ??</skos:prefLabel>
        <skos:prefLabel xml:lang="de">Tag</skos:prefLabel>
        <skos:prefLabel xml:lang="nl">dag</skos:prefLabel>
        <skos:prefLabel xml:lang="en">day</skos:prefLabel>
        <skos:prefLabel xml:lang="pt">dia</skos:prefLabel>
        <skos:prefLabel xml:lang="pl">doba</skos:prefLabel>
        <skos:prefLabel xml:lang="es">d�a</skos:prefLabel>
        <skos:prefLabel xml:lang="it">giorno</skos:prefLabel>
        <skos:prefLabel xml:lang="fr">jour</skos:prefLabel>
    </owl:NamedIndividual>
    


    <!-- http://www.w3.org/2006/time#unitHour -->

    <owl:NamedIndividual rdf:about="http://www.w3.org/2006/time#unitHour">
        <rdf:type rdf:resource="http://www.w3.org/2006/time#TemporalUnit"/>
        <days rdf:datatype="http://www.w3.org/2001/XMLSchema#decimal">0</days>
        <hours rdf:datatype="http://www.w3.org/2001/XMLSchema#decimal">1</hours>
        <minutes rdf:datatype="http://www.w3.org/2001/XMLSchema#decimal">0</minutes>
        <months rdf:datatype="http://www.w3.org/2001/XMLSchema#decimal">0</months>
        <seconds rdf:datatype="http://www.w3.org/2001/XMLSchema#decimal">0</seconds>
        <weeks rdf:datatype="http://www.w3.org/2001/XMLSchema#decimal">0</weeks>
        <years rdf:datatype="http://www.w3.org/2001/XMLSchema#decimal">0</years>
        <rdfs:label xml:lang="en">Hour (unit of temporal duration)</rdfs:label>
        <skos:prefLabel xml:lang="kr">? ??</skos:prefLabel>
        <skos:prefLabel xml:lang="ja">???</skos:prefLabel>
        <skos:prefLabel xml:lang="zh">???</skos:prefLabel>
        <skos:prefLabel>???? ???&quot;@ru</skos:prefLabel>
        <skos:prefLabel xml:lang="ar">???? ?????</skos:prefLabel>
        <skos:prefLabel xml:lang="de">Stunde</skos:prefLabel>
        <skos:prefLabel xml:lang="pl">godzina</skos:prefLabel>
        <skos:prefLabel xml:lang="fr">heure</skos:prefLabel>
        <skos:prefLabel xml:lang="es">hora</skos:prefLabel>
        <skos:prefLabel xml:lang="pt">hora</skos:prefLabel>
        <skos:prefLabel xml:lang="en">hour</skos:prefLabel>
        <skos:prefLabel xml:lang="it">ora</skos:prefLabel>
        <skos:prefLabel xml:lang="nl">uur</skos:prefLabel>
    </owl:NamedIndividual>
    


    <!-- http://www.w3.org/2006/time#unitMinute -->

    <owl:NamedIndividual rdf:about="http://www.w3.org/2006/time#unitMinute">
        <rdf:type rdf:resource="http://www.w3.org/2006/time#TemporalUnit"/>
        <days rdf:datatype="http://www.w3.org/2001/XMLSchema#decimal">0</days>
        <hours rdf:datatype="http://www.w3.org/2001/XMLSchema#decimal">0</hours>
        <minutes rdf:datatype="http://www.w3.org/2001/XMLSchema#decimal">1</minutes>
        <months rdf:datatype="http://www.w3.org/2001/XMLSchema#decimal">0</months>
        <seconds rdf:datatype="http://www.w3.org/2001/XMLSchema#decimal">0</seconds>
        <weeks rdf:datatype="http://www.w3.org/2001/XMLSchema#decimal">0</weeks>
        <years rdf:datatype="http://www.w3.org/2001/XMLSchema#decimal">0</years>
        <rdfs:label xml:lang="en">Minute (unit of temporal duration)</rdfs:label>
        <skos:prefLabel xml:lang="kr">?</skos:prefLabel>
        <skos:prefLabel xml:lang="ja">??</skos:prefLabel>
        <skos:prefLabel xml:lang="zh">???</skos:prefLabel>
        <skos:prefLabel xml:lang="ru">???? ??????</skos:prefLabel>
        <skos:prefLabel xml:lang="ar">????? ?????</skos:prefLabel>
        <skos:prefLabel xml:lang="de">Minute</skos:prefLabel>
        <skos:prefLabel xml:lang="pl">minuta</skos:prefLabel>
        <skos:prefLabel xml:lang="en">minute</skos:prefLabel>
        <skos:prefLabel xml:lang="fr">minute</skos:prefLabel>
        <skos:prefLabel xml:lang="es">minuto</skos:prefLabel>
        <skos:prefLabel xml:lang="it">minuto</skos:prefLabel>
        <skos:prefLabel xml:lang="pt">minuto</skos:prefLabel>
        <skos:prefLabel xml:lang="nl">minuut</skos:prefLabel>
    </owl:NamedIndividual>
    


    <!-- http://www.w3.org/2006/time#unitMonth -->

    <owl:NamedIndividual rdf:about="http://www.w3.org/2006/time#unitMonth">
        <rdf:type rdf:resource="http://www.w3.org/2006/time#TemporalUnit"/>
        <days rdf:datatype="http://www.w3.org/2001/XMLSchema#decimal">0</days>
        <hours rdf:datatype="http://www.w3.org/2001/XMLSchema#decimal">0</hours>
        <minutes rdf:datatype="http://www.w3.org/2001/XMLSchema#decimal">0</minutes>
        <months rdf:datatype="http://www.w3.org/2001/XMLSchema#decimal">1</months>
        <seconds rdf:datatype="http://www.w3.org/2001/XMLSchema#decimal">0</seconds>
        <weeks rdf:datatype="http://www.w3.org/2001/XMLSchema#decimal">0</weeks>
        <years rdf:datatype="http://www.w3.org/2001/XMLSchema#decimal">0</years>
        <rdfs:label xml:lang="en">Month (unit of temporal duration)</rdfs:label>
        <skos:prefLabel xml:lang="kr">??</skos:prefLabel>
        <skos:prefLabel xml:lang="ja">???</skos:prefLabel>
        <skos:prefLabel xml:lang="zh">???</skos:prefLabel>
        <skos:prefLabel xml:lang="ar">??? ????</skos:prefLabel>
        <skos:prefLabel xml:lang="ru">???? ?????</skos:prefLabel>
        <skos:prefLabel xml:lang="de">Monat</skos:prefLabel>
        <skos:prefLabel xml:lang="nl">maand</skos:prefLabel>
        <skos:prefLabel xml:lang="es">mes</skos:prefLabel>
        <skos:prefLabel xml:lang="it">mese</skos:prefLabel>
        <skos:prefLabel xml:lang="pl">miesiac</skos:prefLabel>
        <skos:prefLabel xml:lang="fr">mois</skos:prefLabel>
        <skos:prefLabel xml:lang="en">month</skos:prefLabel>
    </owl:NamedIndividual>
    


    <!-- http://www.w3.org/2006/time#unitSecond -->

    <owl:NamedIndividual rdf:about="http://www.w3.org/2006/time#unitSecond">
        <rdf:type rdf:resource="http://www.w3.org/2006/time#TemporalUnit"/>
        <days rdf:datatype="http://www.w3.org/2001/XMLSchema#decimal">0</days>
        <hours rdf:datatype="http://www.w3.org/2001/XMLSchema#decimal">0</hours>
        <minutes rdf:datatype="http://www.w3.org/2001/XMLSchema#decimal">0</minutes>
        <months rdf:datatype="http://www.w3.org/2001/XMLSchema#decimal">0</months>
        <seconds rdf:datatype="http://www.w3.org/2001/XMLSchema#decimal">1</seconds>
        <weeks rdf:datatype="http://www.w3.org/2001/XMLSchema#decimal">0</weeks>
        <years rdf:datatype="http://www.w3.org/2001/XMLSchema#decimal">0</years>
        <rdfs:label xml:lang="en">Second (unit of temporal duration)</rdfs:label>
        <skos:prefLabel xml:lang="ja">??</skos:prefLabel>
        <skos:prefLabel xml:lang="kr">??</skos:prefLabel>
        <skos:prefLabel xml:lang="zh">??</skos:prefLabel>
        <skos:prefLabel xml:lang="ar">????? ?????</skos:prefLabel>
        <skos:prefLabel xml:lang="de">Sekunde</skos:prefLabel>
        <skos:prefLabel xml:lang="en">second</skos:prefLabel>
        <skos:prefLabel xml:lang="fr">seconde</skos:prefLabel>
        <skos:prefLabel xml:lang="nl">seconde</skos:prefLabel>
        <skos:prefLabel xml:lang="it">secondo</skos:prefLabel>
        <skos:prefLabel xml:lang="es">segundo</skos:prefLabel>
        <skos:prefLabel xml:lang="pt">segundo</skos:prefLabel>
        <skos:prefLabel xml:lang="pl">sekunde</skos:prefLabel>
    </owl:NamedIndividual>
    


    <!-- http://www.w3.org/2006/time#unitWeek -->

    <owl:NamedIndividual rdf:about="http://www.w3.org/2006/time#unitWeek">
        <rdf:type rdf:resource="http://www.w3.org/2006/time#TemporalUnit"/>
        <days rdf:datatype="http://www.w3.org/2001/XMLSchema#decimal">0</days>
        <hours rdf:datatype="http://www.w3.org/2001/XMLSchema#decimal">0</hours>
        <minutes rdf:datatype="http://www.w3.org/2001/XMLSchema#decimal">0</minutes>
        <months rdf:datatype="http://www.w3.org/2001/XMLSchema#decimal">0</months>
        <seconds rdf:datatype="http://www.w3.org/2001/XMLSchema#decimal">0</seconds>
        <weeks rdf:datatype="http://www.w3.org/2001/XMLSchema#decimal">1</weeks>
        <years rdf:datatype="http://www.w3.org/2001/XMLSchema#decimal">0</years>
        <rdfs:label xml:lang="en">Week (unit of temporal duration)</rdfs:label>
        <skos:prefLabel xml:lang="zh">??</skos:prefLabel>
        <skos:prefLabel xml:lang="ja">???</skos:prefLabel>
        <skos:prefLabel xml:lang="kr">???</skos:prefLabel>
        <skos:prefLabel xml:lang="ar">???? ????</skos:prefLabel>
        <skos:prefLabel xml:lang="ru">???? ??????</skos:prefLabel>
        <skos:prefLabel xml:lang="de">Woche</skos:prefLabel>
        <skos:prefLabel xml:lang="fr">semaine</skos:prefLabel>
        <skos:prefLabel xml:lang="es">semana</skos:prefLabel>
        <skos:prefLabel xml:lang="pt">semana</skos:prefLabel>
        <skos:prefLabel xml:lang="it">settimana</skos:prefLabel>
        <skos:prefLabel xml:lang="pl">tydzien</skos:prefLabel>
        <skos:prefLabel xml:lang="en">week</skos:prefLabel>
        <skos:prefLabel xml:lang="nl">week</skos:prefLabel>
    </owl:NamedIndividual>
    


    <!-- http://www.w3.org/2006/time#unitYear -->

    <owl:NamedIndividual rdf:about="http://www.w3.org/2006/time#unitYear">
        <rdf:type rdf:resource="http://www.w3.org/2006/time#TemporalUnit"/>
        <days rdf:datatype="http://www.w3.org/2001/XMLSchema#decimal">0</days>
        <hours rdf:datatype="http://www.w3.org/2001/XMLSchema#decimal">0</hours>
        <minutes rdf:datatype="http://www.w3.org/2001/XMLSchema#decimal">0</minutes>
        <months rdf:datatype="http://www.w3.org/2001/XMLSchema#decimal">0</months>
        <seconds rdf:datatype="http://www.w3.org/2001/XMLSchema#decimal">0</seconds>
        <weeks rdf:datatype="http://www.w3.org/2001/XMLSchema#decimal">0</weeks>
        <years rdf:datatype="http://www.w3.org/2001/XMLSchema#decimal">1</years>
        <rdfs:label xml:lang="en">Year (unit of temporal duration)</rdfs:label>
        <skos:prefLabel xml:lang="kr">1 ?</skos:prefLabel>
        <skos:prefLabel xml:lang="ja">??</skos:prefLabel>
        <skos:prefLabel xml:lang="zh">??</skos:prefLabel>
        <skos:prefLabel xml:lang="ar">??? ?????</skos:prefLabel>
        <skos:prefLabel xml:lang="ru">???? ???</skos:prefLabel>
        <skos:prefLabel xml:lang="de">Jahr</skos:prefLabel>
        <skos:prefLabel xml:lang="fr">an</skos:prefLabel>
        <skos:prefLabel xml:lang="it">anno</skos:prefLabel>
        <skos:prefLabel xml:lang="pt">ano</skos:prefLabel>
        <skos:prefLabel xml:lang="nl">jaar</skos:prefLabel>
        <skos:prefLabel xml:lang="pl">rok</skos:prefLabel>
        <skos:prefLabel xml:lang="es">un a�o</skos:prefLabel>
        <skos:prefLabel xml:lang="en">year</skos:prefLabel>
    </owl:NamedIndividual>
    <rdf:Description>
        <xsd:pattern>--(0[1-9]|1[0-9]|20)(Z|(\+|-)((0[0-9]|1[0-3]):[0-5][0-9]|14:00))?</xsd:pattern>
    </rdf:Description>
    <rdf:Description>
        <xsd:pattern>---(0[1-9]|[1-9][0-9])(Z|(\+|-)((0[0-9]|1[0-3]):[0-5][0-9]|14:00))?</xsd:pattern>
    </rdf:Description>
    <rdf:Description>
        <xsd:pattern>-?([1-9][0-9]{3,}|0[0-9]{3})(Z|(\+|-)((0[0-9]|1[0-3]):[0-5][0-9]|14:00))?</xsd:pattern>
    </rdf:Description>
</rdf:RDF>



<!-- Generated by the OWL API (version 4.5.9.2019-02-01T07:24:44Z) https://github.com/owlcs/owlapi -->

